lunarlander_sl/SmallStep.thy
@@ -14,19 +14,19 @@ inductive small_step :: "proc \<Rightarrow> state \<Rightarrow> trace_block opti
 | seqS2: "small_step (Seq Skip c) s None c s"
 | condS1: "b s \<Longrightarrow> small_step (Cond b c1 c2) s None c1 s"
 | condS2: "\<not>b s \<Longrightarrow> small_step (Cond b c1 c2) s None c2 s"
-| waitS1: "d1 > 0 \<Longrightarrow> d1 < d \<Longrightarrow> small_step (Wait d) s (Some (WaitBlock d1 (\<lambda>\<tau>\<in>{0..d1}. State s) ({}, {})))
+| waitS1: "d1 > 0 \<Longrightarrow> d1 < d \<Longrightarrow> small_step (Wait d) s (Some (WaitBlk d1 (\<lambda>_. State s) ({}, {})))
                                  (Wait (d - d1)) s"
-| waitS2: "d > 0 \<Longrightarrow> small_step (Wait d) s (Some (WaitBlock d (\<lambda>\<tau>\<in>{0..d}. State s) ({}, {}))) Skip s"
+| waitS2: "d > 0 \<Longrightarrow> small_step (Wait d) s (Some (WaitBlk d (\<lambda>_. State s) ({}, {}))) Skip s"
 | waitS3: "\<not>d > 0 \<Longrightarrow> small_step (Wait d) s None Skip s"
 | sendS1: "small_step (Cm (ch[!]e)) s (Some (OutBlock ch (e s))) Skip s"
-| sendS2: "d > 0 \<Longrightarrow> small_step (Cm (ch[!]e)) s (Some (WaitBlock d (\<lambda>\<tau>\<in>{0..d}. State s) ({ch}, {})))
+| sendS2: "d > 0 \<Longrightarrow> small_step (Cm (ch[!]e)) s (Some (WaitBlk d (\<lambda>_. State s) ({ch}, {})))
                                 (Cm (ch[!]e)) s"
 | receiveS1: "small_step (Cm (ch[?]var)) s (Some (InBlock ch v)) Skip (s(var := v))"
-| receiveS2: "d > 0 \<Longrightarrow> small_step (Cm (ch[?]var)) s (Some (WaitBlock d (\<lambda>\<tau>\<in>{0..d}. State s) ({}, {ch})))
+| receiveS2: "d > 0 \<Longrightarrow> small_step (Cm (ch[?]var)) s (Some (WaitBlk d (\<lambda>_. State s) ({}, {ch})))
                                    (Cm (ch[?]var)) s"
 | IChoiceS1: "small_step (IChoice p1 p2) s None p1 s"
 | IChoiceS2: "small_step (IChoice p1 p2) s None p2 s"
-| EChoiceS1: "d > 0 \<Longrightarrow> small_step (EChoice cs) s (Some (WaitBlock d (\<lambda>\<tau>\<in>{0..d}. State s) (rdy_of_echoice cs)))
+| EChoiceS1: "d > 0 \<Longrightarrow> small_step (EChoice cs) s (Some (WaitBlk d (\<lambda>_. State s) (rdy_of_echoice cs)))
                                    (EChoice cs) s"
 | EChoiceS2: "i < length cs \<Longrightarrow> cs ! i = (Send ch e, p2) \<Longrightarrow>
     small_step (EChoice cs) s (Some (OutBlock ch (e s))) p2 s"
@@ -36,12 +36,12 @@ inductive small_step :: "proc \<Rightarrow> state \<Rightarrow> trace_block opti
 | RepetitionS2: "small_step (Rep p) s None (Seq p (Rep p)) s"
 | ContS1: "d > 0 \<Longrightarrow> ODEsol ode p d \<Longrightarrow>
     (\<forall>t. t \<ge> 0 \<and> t < d \<longrightarrow> b (p t)) \<Longrightarrow>
-    p 0 = s \<Longrightarrow> small_step (Cont ode b) s (Some (WaitBlock d (\<lambda>\<tau>\<in>{0..d}. State (p \<tau>)) ({}, {})))
+    p 0 = s \<Longrightarrow> small_step (Cont ode b) s (Some (WaitBlk d (\<lambda>\<tau>. State (p \<tau>)) ({}, {})))
                            (Cont ode b) (p d)"
 | ContS2: "\<not>b s \<Longrightarrow> small_step (Cont ode b) s None Skip s"
 | InterruptS1: "d > 0 \<Longrightarrow> ODEsol ode p d \<Longrightarrow>
     (\<forall>t. t \<ge> 0 \<and> t < d \<longrightarrow> b (p t)) \<Longrightarrow>
-    p 0 = s \<Longrightarrow> small_step (Interrupt ode b cs) s (Some (WaitBlock d (\<lambda>\<tau>\<in>{0..d}. State (p \<tau>)) (rdy_of_echoice cs)))
+    p 0 = s \<Longrightarrow> small_step (Interrupt ode b cs) s (Some (WaitBlk d (\<lambda>\<tau>. State (p \<tau>)) (rdy_of_echoice cs)))
                            (Interrupt ode b cs) (p d)"
 | InterruptS2: "\<not>b s \<Longrightarrow> small_step (Interrupt ode b cs) s None Skip s"
 | InterruptS3: "i < length cs \<Longrightarrow> cs ! i = (Send ch e, p2) \<Longrightarrow>
@@ -64,8 +64,8 @@ text \<open>Further, we define equivalence between two traces\<close>
 inductive reduce_trace :: "trace \<Rightarrow> trace \<Rightarrow> bool" where
   reduce_trace_empty: "reduce_trace [] []"
 | reduce_trace_merge: "d1 > 0 \<Longrightarrow> d2 > 0 \<Longrightarrow> p1 d1 = p2 0 \<Longrightarrow>
-   reduce_trace (WaitBlock d1 (\<lambda>\<tau>\<in>{0..d1}. p1 \<tau>) rdy # WaitBlock d2 (\<lambda>\<tau>\<in>{0..d2}. p2 \<tau>) rdy # tr)
-               (WaitBlock (d1 + d2) (\<lambda>\<tau>\<in>{0..d1+d2}. if \<tau> < d1 then p1 \<tau> else p2 (\<tau> - d1)) rdy # tr)"
+   reduce_trace (WaitBlk d1 p1 rdy # WaitBlk d2 p2 rdy # tr)
+               (WaitBlk (d1 + d2) (\<lambda>\<tau>. if \<tau> < d1 then p1 \<tau> else p2 (\<tau> - d1)) rdy # tr)"
 | reduce_trace_cons: "reduce_trace tr1 tr2 \<Longrightarrow> reduce_trace (ev # tr1) (ev # tr2)"
 | reduce_trace_trans: "reduce_trace tr1 tr2 \<Longrightarrow> reduce_trace tr2 tr3 \<Longrightarrow> reduce_trace tr1 tr3"
 
@@ -121,13 +121,13 @@ lemma reduce_trace_merge':
   assumes "d1 > 0" "d2 > 0"
    "\<forall>\<tau>\<in>{0..d1}. hist1 \<tau> = hist \<tau>"
    "\<forall>\<tau>\<in>{0..d2}. hist2 \<tau> = hist (\<tau> + d1)"
-  shows "reduce_trace (WaitBlock d1 (\<lambda>\<tau>\<in>{0..d1}. hist1 \<tau>) rdy # WaitBlock d2 (\<lambda>\<tau>\<in>{0..d2}. hist2 \<tau>) rdy # tr)
-                     (WaitBlock (d1 + d2) (\<lambda>\<tau>\<in>{0..d1+d2}. hist \<tau>) rdy # tr)"
+  shows "reduce_trace (WaitBlk d1 hist1 rdy # WaitBlk d2 hist2 rdy # tr)
+                      (WaitBlk (d1 + d2) hist rdy # tr)"
 proof -
   have a: "(\<lambda>\<tau>\<in>{0..d1+d2}. hist \<tau>) = (\<lambda>\<tau>\<in>{0..d1+d2}. if \<tau> < d1 then hist1 \<tau> else hist2 (\<tau> - d1))"
     using assms by auto
   show ?thesis
-    unfolding a apply (rule reduce_trace_merge)
+    unfolding WaitBlk_def a apply (rule reduce_trace_merge[unfolded WaitBlk_def])
     using assms by auto
 qed
 
@@ -403,15 +403,15 @@ proof (induction arbitrary: tr2 s3 rule: small_step.induct)
     by (rule seqB[OF b(2) a(3)])
 next
   case (waitS1 d1 d s)
-  have a: "tr2 = [WaitBlock (d - d1) (\<lambda>\<tau>\<in>{0..d - d1}. State s) ({}, {})]" "s3 = s" "0 < d - d1"
+  have a: "tr2 = [WaitBlk (d - d1) (\<lambda>_. State s) ({}, {})]" "s3 = s" "0 < d - d1"
     using waitE[OF waitS1(4)] by (auto simp add: waitS1(1,2))
-  have b: "ev = WaitBlock d1 (\<lambda>\<tau>\<in>{0..d1}. State s) ({}, {})"
+  have b: "ev = WaitBlk d1 (\<lambda>_. State s) ({}, {})"
     using waitS1(3) by auto
-  have c: "WaitBlock d (\<lambda>\<tau>\<in>{0..d}. State s) ({}, {}) =
-           WaitBlock (d1 + (d - d1)) (\<lambda>\<tau>\<in>{0..d1+(d-d1)}. if \<tau> < d1 then State s else State s) ({}, {})"
+  have c: "WaitBlk d (\<lambda>_. State s) ({}, {}) =
+           WaitBlk (d1 + (d - d1)) (\<lambda>\<tau>. if \<tau> < d1 then State s else State s) ({}, {})"
     by auto
   show ?case
-    apply (rule exI[where x="[WaitBlock d (\<lambda>\<tau>\<in>{0..d}. State s) ({}, {})]"])
+    apply (rule exI[where x="[WaitBlk d (\<lambda>_. State s) ({}, {})]"])
     unfolding a b apply auto
     unfolding c apply (rule reduce_trace_merge)
        apply (auto simp add: waitS1)
@@ -419,7 +419,7 @@ next
     using waitS1 by auto
 next
   case (waitS2 d s)
-  have a: "ev = WaitBlock d (\<lambda>\<tau>\<in>{0..d}. State s) ({}, {})"
+  have a: "ev = WaitBlk d (\<lambda>_. State s) ({}, {})"
     using waitS2(2) by auto
   have b: "tr2 = []"
     using waitS2(3) apply (rule skipE) by auto
@@ -427,7 +427,7 @@ next
     using waitS2(3) apply (rule skipE) by auto
   show ?case
     unfolding a b c
-    apply (rule exI[where x="[WaitBlock d (\<lambda>\<tau>\<in>{0..d}. State s) ({}, {})]"])
+    apply (rule exI[where x="[WaitBlk d (\<lambda>_. State s) ({}, {})]"])
     apply auto
     apply (rule waitB1) by (rule waitS2(1))
 next
@@ -445,12 +445,12 @@ next
     by (rule sendB1)
 next
   case (sendS2 d ch e s)
-  have a: "ev = WaitBlock d (\<lambda>\<tau>\<in>{0..d}. State s) ({ch}, {})"
+  have a: "ev = WaitBlk d (\<lambda>_. State s) ({ch}, {})"
     using sendS2(2) by auto
-  have b: "reduce_trace [WaitBlock d (\<lambda>\<tau>\<in>{0..d}. State s) ({ch}, {}), WaitBlock d2 (\<lambda>\<tau>\<in>{0..d2}. State s) ({ch}, {}), OutBlock ch (e s)]
-           [WaitBlock (d + d2) (\<lambda>\<tau>\<in>{0..d + d2}. State s) ({ch}, {}), OutBlock ch (e s)]" (is "reduce_trace ?lhs ?rhs") if "d2 > 0" for d2
+  have b: "reduce_trace [WaitBlk d (\<lambda>_. State s) ({ch}, {}), WaitBlk d2 (\<lambda>_. State s) ({ch}, {}), OutBlock ch (e s)]
+           [WaitBlk (d + d2) (\<lambda>_. State s) ({ch}, {}), OutBlock ch (e s)]" (is "reduce_trace ?lhs ?rhs") if "d2 > 0" for d2
   proof -
-    have b2: "?rhs = [WaitBlock (d + d2) (\<lambda>\<tau>\<in>{0..d + d2}. if \<tau> < d then State s else State s) ({ch}, {}), OutBlock ch (e s)]"
+    have b2: "?rhs = [WaitBlk (d + d2) (\<lambda>\<tau>. if \<tau> < d then State s else State s) ({ch}, {}), OutBlock ch (e s)]"
       by auto
     show ?thesis
       unfolding b2 apply (rule reduce_trace_merge)
@@ -459,11 +459,11 @@ next
   show ?case
     using sendS2(3) apply (elim sendE)
     subgoal
-      apply (rule exI[where x="[WaitBlock d (\<lambda>\<tau>\<in>{0..d}. State s) ({ch}, {}), OutBlock ch (e s)]"])
+      apply (rule exI[where x="[WaitBlk d (\<lambda>_. State s) ({ch}, {}), OutBlock ch (e s)]"])
       apply (auto simp add: a)
       apply (rule sendB2) by (rule sendS2(1))
     subgoal for d2
-      apply (rule exI[where x="[WaitBlock (d + d2) (\<lambda>\<tau>\<in>{0..d+d2}. State s) ({ch}, {}), OutBlock ch (e s)]"])
+      apply (rule exI[where x="[WaitBlk (d + d2) (\<lambda>_. State s) ({ch}, {}), OutBlock ch (e s)]"])
       apply (auto simp add: a)
       subgoal by (rule b)
       apply (rule sendB2) using sendS2(1) by auto
@@ -482,12 +482,12 @@ next
     using reduce_trace_refl receiveB1 by blast
 next
   case (receiveS2 d ch var s)
-  have a: "ev = WaitBlock d (\<lambda>\<tau>\<in>{0..d}. State s) ({}, {ch})"
+  have a: "ev = WaitBlk d (\<lambda>_. State s) ({}, {ch})"
     using receiveS2(2) by auto
-  have b: "reduce_trace [WaitBlock d (\<lambda>\<tau>\<in>{0..d}. State s) ({}, {ch}), WaitBlock d2 (\<lambda>\<tau>\<in>{0..d2}. State s) ({}, {ch}), InBlock ch v]
-           [WaitBlock (d + d2) (\<lambda>\<tau>\<in>{0..d + d2}. State s) ({}, {ch}), InBlock ch v]" (is "reduce_trace ?lhs ?rhs") if "d2 > 0" for v d2
+  have b: "reduce_trace [WaitBlk d (\<lambda>_. State s) ({}, {ch}), WaitBlk d2 (\<lambda>_. State s) ({}, {ch}), InBlock ch v]
+           [WaitBlk (d + d2) (\<lambda>_. State s) ({}, {ch}), InBlock ch v]" (is "reduce_trace ?lhs ?rhs") if "d2 > 0" for v d2
   proof -
-    have b2: "?rhs = [WaitBlock (d + d2) (\<lambda>\<tau>\<in>{0..d + d2}. if \<tau> < d then State s else State s) ({}, {ch}), InBlock ch v]"
+    have b2: "?rhs = [WaitBlk (d + d2) (\<lambda>\<tau>. if \<tau> < d then State s else State s) ({}, {ch}), InBlock ch v]"
       by auto
     show ?thesis
       unfolding b2 apply (rule reduce_trace_merge)
@@ -496,12 +496,12 @@ next
   show ?case
     using receiveS2(3) apply (elim receiveE)
     subgoal for v
-      apply (rule exI[where x="[WaitBlock d (\<lambda>\<tau>\<in>{0..d}. State s) ({}, {ch}), InBlock ch v]"])
+      apply (rule exI[where x="[WaitBlk d (\<lambda>_. State s) ({}, {ch}), InBlock ch v]"])
       apply (auto simp add: a)
       apply (subst fun_upd_def[symmetric])
       apply (rule receiveB2) by (rule receiveS2(1))
     subgoal for d2 v
-      apply (rule exI[where x="[WaitBlock (d + d2) (\<lambda>\<tau>\<in>{0..d+d2}. State s) ({}, {ch}), InBlock ch v]"])
+      apply (rule exI[where x="[WaitBlk (d + d2) (\<lambda>_. State s) ({}, {ch}), InBlock ch v]"])
       apply (auto simp add: a)
       subgoal by (rule b)
       apply (subst fun_upd_def[symmetric])
@@ -509,15 +509,15 @@ next
     done
 next
   case (EChoiceS1 d cs s)
-  have a: "ev = WaitBlock d (\<lambda>\<tau>\<in>{0..d}. State s) (rdy_of_echoice cs)"
+  have a: "ev = WaitBlk d (\<lambda>_. State s) (rdy_of_echoice cs)"
     using EChoiceS1(2) by auto
   have b: "reduce_trace
-     (WaitBlock d (\<lambda>\<tau>\<in>{0..d}. State s) (rdy_of_echoice cs) #
-      WaitBlock d2 (\<lambda>\<tau>\<in>{0..d2}. State s) (rdy_of_echoice cs) # OutBlock ch (e s) # tr2')
-     (WaitBlock (d + d2) (\<lambda>\<tau>\<in>{0..d + d2}. State s) (rdy_of_echoice cs) # OutBlock ch (e s) # tr2')"
+     (WaitBlk d (\<lambda>_. State s) (rdy_of_echoice cs) #
+      WaitBlk d2 (\<lambda>_. State s) (rdy_of_echoice cs) # OutBlock ch (e s) # tr2')
+     (WaitBlk (d + d2) (\<lambda>_. State s) (rdy_of_echoice cs) # OutBlock ch (e s) # tr2')"
     (is "reduce_trace ?lhs ?rhs") if "d2 > 0" for d2 ch e tr2'
   proof -
-    have b2: "?rhs = WaitBlock (d + d2) (\<lambda>\<tau>\<in>{0..d + d2}. if \<tau> < d then State s else State s) (rdy_of_echoice cs) #
+    have b2: "?rhs = WaitBlk (d + d2) (\<lambda>\<tau>. if \<tau> < d then State s else State s) (rdy_of_echoice cs) #
                      OutBlock ch (e s) # tr2'"
       by auto
     show ?thesis
@@ -525,12 +525,12 @@ next
       by (auto simp add: EChoiceS1 that)
   qed
   have c: "reduce_trace
-     (WaitBlock d (\<lambda>\<tau>\<in>{0..d}. State s) (rdy_of_echoice cs) #
-      WaitBlock d2 (\<lambda>\<tau>\<in>{0..d2}. State s) (rdy_of_echoice cs) # InBlock ch v # tr2')
-     (WaitBlock (d + d2) (\<lambda>\<tau>\<in>{0..d + d2}. State s) (rdy_of_echoice cs) # InBlock ch v # tr2')"
+     (WaitBlk d (\<lambda>_. State s) (rdy_of_echoice cs) #
+      WaitBlk d2 (\<lambda>_. State s) (rdy_of_echoice cs) # InBlock ch v # tr2')
+     (WaitBlk (d + d2) (\<lambda>_. State s) (rdy_of_echoice cs) # InBlock ch v # tr2')"
     (is "reduce_trace ?lhs ?rhs") if "d2 > 0" for d2 ch v tr2'
   proof -
-    have c2: "?rhs = WaitBlock (d + d2) (\<lambda>\<tau>\<in>{0..d + d2}. if \<tau> < d then State s else State s) (rdy_of_echoice cs) # InBlock ch v # tr2'"
+    have c2: "?rhs = WaitBlk (d + d2) (\<lambda>\<tau>. if \<tau> < d then State s else State s) (rdy_of_echoice cs) # InBlock ch v # tr2'"
       by auto
     show ?thesis
       unfolding c2 apply (rule reduce_trace_merge)
@@ -539,21 +539,21 @@ next
   show ?case
     using EChoiceS1(3) apply (elim echoiceE)
     subgoal for i ch e p2 tr2'
-      apply (rule exI[where x="WaitBlock d (\<lambda>\<tau>\<in>{0..d}. State s) (rdy_of_echoice cs) # OutBlock ch (e s) # tr2'"])
+      apply (rule exI[where x="WaitBlk d (\<lambda>_. State s) (rdy_of_echoice cs) # OutBlock ch (e s) # tr2'"])
       unfolding a apply auto apply (rule EChoiceSendB2)
       by (auto simp add: EChoiceS1)
     subgoal for d2 i ch e p2 tr2'
-      apply (rule exI[where x="WaitBlock (d + d2) (\<lambda>\<tau>\<in>{0..d+d2}. State s) (rdy_of_echoice cs) # OutBlock ch (e s) # tr2'"])
+      apply (rule exI[where x="WaitBlk (d + d2) (\<lambda>_. State s) (rdy_of_echoice cs) # OutBlock ch (e s) # tr2'"])
       unfolding a apply auto subgoal by (rule b)
       apply (rule EChoiceSendB2)
          apply (auto simp add: EChoiceS1)
       using EChoiceS1(1) by auto
     subgoal for i ch var p2 v tr2'
-      apply (rule exI[where x="WaitBlock d (\<lambda>\<tau>\<in>{0..d}. State s) (rdy_of_echoice cs) # InBlock ch v # tr2'"])
+      apply (rule exI[where x="WaitBlk d (\<lambda>_. State s) (rdy_of_echoice cs) # InBlock ch v # tr2'"])
       unfolding a apply auto apply (rule EChoiceReceiveB2)
       by (auto simp add: EChoiceS1)
     subgoal for d2 i ch var p2 v tr2'
-      apply (rule exI[where x="WaitBlock (d + d2) (\<lambda>\<tau>\<in>{0..d+d2}. State s) (rdy_of_echoice cs) # InBlock ch v # tr2'"])
+      apply (rule exI[where x="WaitBlk (d + d2) (\<lambda>_. State s) (rdy_of_echoice cs) # InBlock ch v # tr2'"])
       unfolding a apply auto subgoal by (rule c)
       apply (rule EChoiceReceiveB2)
          apply (auto simp add: EChoiceS1)
@@ -579,9 +579,9 @@ next
     by (rule EChoiceReceiveB1[OF EChoiceS3(1,2,4)])
 next
   case (ContS1 d ode p b s)
-  have a: "ev = WaitBlock d (\<lambda>\<tau>\<in>{0..d}. State (p \<tau>)) ({}, {})"
+  have a: "ev = WaitBlk d (\<lambda>\<tau>. State (p \<tau>)) ({}, {})"
     using ContS1(5) by auto
-  have b: "big_step (Cont ode b) s [WaitBlock (d + d2) (\<lambda>\<tau>\<in>{0..d + d2}. State (if \<tau> < d then p \<tau> else p2 (\<tau> - d))) ({}, {})] (p2 d2)"
+  have b: "big_step (Cont ode b) s [WaitBlk (d + d2) (\<lambda>\<tau>. State (if \<tau> < d then p \<tau> else p2 (\<tau> - d))) ({}, {})] (p2 d2)"
     if "d2 > 0" "ODEsol ode p2 d2" "\<forall>t. 0 \<le> t \<and> t < d2 \<longrightarrow> b (p2 t)" "\<not> b (p2 d2)" "p2 0 = p d" for p2 d2
   proof -
     let ?p3="\<lambda>\<tau>. if \<tau> < d then p \<tau> else p2 (\<tau> - d)"
@@ -596,12 +596,12 @@ next
       subgoal using ContS1(1,4) by auto
       done
   qed
-  have c: "reduce_trace [WaitBlock d (\<lambda>\<tau>\<in>{0..d}. State (p \<tau>)) ({}, {}), WaitBlock d2 (\<lambda>\<tau>\<in>{0..d2}. State (p2 \<tau>)) ({}, {})]
-     [WaitBlock (d + d2) (\<lambda>\<tau>\<in>{0..d + d2}. State (if \<tau> < d then p \<tau> else p2 (\<tau> - d))) ({}, {})]"
+  have c: "reduce_trace [WaitBlk d (\<lambda>\<tau>. State (p \<tau>)) ({}, {}), WaitBlk d2 (\<lambda>\<tau>. State (p2 \<tau>)) ({}, {})]
+     [WaitBlk (d + d2) (\<lambda>\<tau>. State (if \<tau> < d then p \<tau> else p2 (\<tau> - d))) ({}, {})]"
     (is "reduce_trace ?lhs ?rhs") if "p2 0 = p d" "d2 > 0" for d2 p2       
   proof -
-    have c1: "?rhs = [WaitBlock (d + d2) (\<lambda>\<tau>\<in>{0..d + d2}. if \<tau> < d then State (p \<tau>) else State (p2 (\<tau> - d))) ({}, {})]"
-      by auto
+    have c1: "?rhs = [WaitBlk (d + d2) (\<lambda>\<tau>. if \<tau> < d then State (p \<tau>) else State (p2 (\<tau> - d))) ({}, {})]"
+      by (auto simp add: WaitBlk_def)
     show ?thesis
       unfolding c1 apply (rule reduce_trace_merge)
       by (auto simp add: that ContS1)
@@ -609,21 +609,21 @@ next
   show ?case
     using ContS1(6) apply (elim contE)
     subgoal
-      apply (rule exI[where x="[WaitBlock d (\<lambda>\<tau>\<in>{0..d}. State (p \<tau>)) ({}, {})]"])
+      apply (rule exI[where x="[WaitBlk d (\<lambda>\<tau>. State (p \<tau>)) ({}, {})]"])
       unfolding a apply auto
       apply (rule ContB2) using ContS1 by auto
     subgoal for d2 p2
-      apply (rule exI[where x="[WaitBlock (d + d2) (\<lambda>\<tau>\<in>{0..d+d2}. State (if \<tau> < d then p \<tau> else p2 (\<tau> - d))) ({}, {})]"])
+      apply (rule exI[where x="[WaitBlk (d + d2) (\<lambda>\<tau>. State (if \<tau> < d then p \<tau> else p2 (\<tau> - d))) ({}, {})]"])
       unfolding a apply auto
       subgoal by (rule c)
       using b by auto
     done
 next
   case (InterruptS1 d ode p b s cs)
-  have a: "ev = WaitBlock d (\<lambda>\<tau>\<in>{0..d}. State (p \<tau>)) (rdy_of_echoice cs)"
+  have a: "ev = WaitBlk d (\<lambda>\<tau>. State (p \<tau>)) (rdy_of_echoice cs)"
     using InterruptS1(5) by auto
   have b: "big_step (Interrupt ode b cs) s
-     (WaitBlock (d + d2) (\<lambda>\<tau>\<in>{0..d + d2}. State (if \<tau> < d then p \<tau> else p2 (\<tau> - d))) (rdy_of_echoice cs) # OutBlock ch (e (p2 d2)) # tr2') s3"
+     (WaitBlk (d + d2) (\<lambda>\<tau>. State (if \<tau> < d then p \<tau> else p2 (\<tau> - d))) (rdy_of_echoice cs) # OutBlock ch (e (p2 d2)) # tr2') s3"
     if "d2 > 0" "ODEsol ode p2 d2" "p2 0 = p d" "\<forall>t. 0 \<le> t \<and> t < d2 \<longrightarrow> b (p2 t)"
        "i < length cs" "cs ! i = (ch[!]e, p3)" "big_step p3 (p2 d2) tr2' s3" for d2 p2 ch e tr2' i p3
   proof -
@@ -641,7 +641,7 @@ next
       done 
   qed
   have c: "big_step (Interrupt ode b cs) s
-     (WaitBlock (d + d2) (\<lambda>\<tau>\<in>{0..d + d2}. State (if \<tau> < d then p \<tau> else p2 (\<tau> - d))) (rdy_of_echoice cs) # InBlock ch v # tr2') s3"
+     (WaitBlk (d + d2) (\<lambda>\<tau>. State (if \<tau> < d then p \<tau> else p2 (\<tau> - d))) (rdy_of_echoice cs) # InBlock ch v # tr2') s3"
     if "0 < d2" "ODEsol ode p2 d2" "p2 0 = p d" "\<forall>t. 0 \<le> t \<and> t < d2 \<longrightarrow> b (p2 t)"
        "i < length cs" "cs ! i = (ch[?]var, p3)" "big_step p3 ((p2 d2)(var := v)) tr2' s3" for d2 p2 ch v tr2' i var p3
   proof -
@@ -659,7 +659,7 @@ next
       done
   qed
   have d: "big_step (Interrupt ode b cs) s
-     [WaitBlock (d + d2) (\<lambda>\<tau>\<in>{0..d + d2}. State (if \<tau> < d then p \<tau> else p2 (\<tau> - d))) (rdy_of_echoice cs)] (p2 d2)"
+     [WaitBlk (d + d2) (\<lambda>\<tau>. State (if \<tau> < d then p \<tau> else p2 (\<tau> - d))) (rdy_of_echoice cs)] (p2 d2)"
     if "0 < d2" "ODEsol ode p2 d2" "\<forall>t. 0 \<le> t \<and> t < d2 \<longrightarrow> b (p2 t)" "\<not> b (p2 d2)" "p2 0 = p d" for d2 p2
   proof -
     let ?p3="\<lambda>\<tau>. if \<tau> < d then p \<tau> else p2 (\<tau> - d)"
@@ -675,36 +675,37 @@ next
       by auto
   qed
   have e: "reduce_trace
-     (WaitBlock d (\<lambda>\<tau>\<in>{0..d}. State (p \<tau>)) (rdy_of_echoice cs) #
-      WaitBlock d2 (\<lambda>\<tau>\<in>{0..d2}. State (p2 \<tau>)) (rdy_of_echoice cs) # OutBlock ch (e (p2 d2)) # tr2')
-     (WaitBlock (d + d2) (\<lambda>\<tau>\<in>{0..d + d2}. State (if \<tau> < d then p \<tau> else p2 (\<tau> - d))) (rdy_of_echoice cs) # OutBlock ch (e (p2 d2)) # tr2')"
+     (WaitBlk d (\<lambda>\<tau>. State (p \<tau>)) (rdy_of_echoice cs) #
+      WaitBlk d2 (\<lambda>\<tau>. State (p2 \<tau>)) (rdy_of_echoice cs) # OutBlock ch (e (p2 d2)) # tr2')
+     (WaitBlk (d + d2) (\<lambda>\<tau>. State (if \<tau> < d then p \<tau> else p2 (\<tau> - d))) (rdy_of_echoice cs) # OutBlock ch (e (p2 d2)) # tr2')"
     (is "reduce_trace ?lhs ?rhs") if "p2 0 = p d" "d2 > 0" for d2 p2 ch e tr2'
   proof -
-    have e2: "?rhs = WaitBlock (d + d2) (\<lambda>\<tau>\<in>{0..d + d2}. if \<tau> < d then State (p \<tau>) else State (p2 (\<tau> - d))) (rdy_of_echoice cs) #
+    have e2: "?rhs = WaitBlk (d + d2) (\<lambda>\<tau>. if \<tau> < d then State (p \<tau>) else State (p2 (\<tau> - d))) (rdy_of_echoice cs) #
                      OutBlock ch (e (p2 d2)) # tr2'"
-      by auto
+      by (auto simp add: WaitBlk_def)
     show ?thesis
       unfolding e2 apply (rule reduce_trace_merge)
       by (auto simp add: InterruptS1 that)
   qed
   have f: "reduce_trace
-     (WaitBlock d (\<lambda>\<tau>\<in>{0..d}. State (p \<tau>)) (rdy_of_echoice cs) # WaitBlock d2 (\<lambda>\<tau>\<in>{0..d2}. State (p2 \<tau>)) (rdy_of_echoice cs) # InBlock ch v # tr2')
-     (WaitBlock (d + d2) (\<lambda>\<tau>\<in>{0..d + d2}. State (if \<tau> < d then p \<tau> else p2 (\<tau> - d))) (rdy_of_echoice cs) # InBlock ch v # tr2')"
+     (WaitBlk d (\<lambda>\<tau>. State (p \<tau>)) (rdy_of_echoice cs) # WaitBlk d2 (\<lambda>\<tau>. State (p2 \<tau>)) (rdy_of_echoice cs) # InBlock ch v # tr2')
+     (WaitBlk (d + d2) (\<lambda>\<tau>. State (if \<tau> < d then p \<tau> else p2 (\<tau> - d))) (rdy_of_echoice cs) # InBlock ch v # tr2')"
     (is "reduce_trace ?lhs ?rhs") if "p2 0 = p d" "d2 > 0" for d2 p2 ch v tr2'
   proof -
-    have f2: "?rhs = WaitBlock (d + d2) (\<lambda>\<tau>\<in>{0..d + d2}. if \<tau> < d then State (p \<tau>) else State (p2 (\<tau> - d))) (rdy_of_echoice cs) #
+    have f2: "?rhs = WaitBlk (d + d2) (\<lambda>\<tau>. if \<tau> < d then State (p \<tau>) else State (p2 (\<tau> - d))) (rdy_of_echoice cs) #
                      InBlock ch v # tr2'"
-      by auto
+      by (auto simp add: WaitBlk_def)
     show ?thesis
       unfolding f2 apply (rule reduce_trace_merge)
       by (auto simp add: that InterruptS1)
   qed
-  have g: "reduce_trace [WaitBlock d (\<lambda>\<tau>\<in>{0..d}. State (p \<tau>)) (rdy_of_echoice cs), WaitBlock d2 (\<lambda>\<tau>\<in>{0..d2}. State (p2 \<tau>)) (rdy_of_echoice cs)]
-     [WaitBlock (d + d2) (\<lambda>\<tau>\<in>{0..d + d2}. State (if \<tau> < d then p \<tau> else p2 (\<tau> - d))) (rdy_of_echoice cs)]"
+  have g: "reduce_trace [WaitBlk d (\<lambda>\<tau>. State (p \<tau>)) (rdy_of_echoice cs),
+                         WaitBlk d2 (\<lambda>\<tau>. State (p2 \<tau>)) (rdy_of_echoice cs)]
+     [WaitBlk (d + d2) (\<lambda>\<tau>. State (if \<tau> < d then p \<tau> else p2 (\<tau> - d))) (rdy_of_echoice cs)]"
     (is "reduce_trace ?lhs ?rhs") if "p2 0 = p d" "d2 > 0" for d2 p2
   proof -
-    have g1: "?rhs = [WaitBlock (d + d2) (\<lambda>\<tau>\<in>{0..d + d2}. if \<tau> < d then State (p \<tau>) else State (p2 (\<tau> - d))) (rdy_of_echoice cs)]"
-      by auto
+    have g1: "?rhs = [WaitBlk (d + d2) (\<lambda>\<tau>. if \<tau> < d then State (p \<tau>) else State (p2 (\<tau> - d))) (rdy_of_echoice cs)]"
+      by (auto simp add: WaitBlk_def)
     show ?thesis
       unfolding g1 apply (rule reduce_trace_merge)
       by (auto simp add: that InterruptS1)
@@ -712,32 +713,32 @@ next
   show ?case
     using InterruptS1(6) apply (elim interruptE)
     subgoal for i ch e p2 tr2'
-      apply (rule exI[where x="WaitBlock d (\<lambda>\<tau>\<in>{0..d}. State (p \<tau>)) (rdy_of_echoice cs) # OutBlock ch (e (p d)) # tr2'"])
+      apply (rule exI[where x="WaitBlk d (\<lambda>\<tau>. State (p \<tau>)) (rdy_of_echoice cs) # OutBlock ch (e (p d)) # tr2'"])
       unfolding a apply auto apply (rule InterruptSendB2)
       by (auto simp add: InterruptS1)
     subgoal for d2 p2 i ch e p3 tr2'
-      apply (rule exI[where x="WaitBlock (d + d2) (\<lambda>\<tau>\<in>{0..d+d2}. State (if \<tau> < d then p \<tau> else p2 (\<tau> - d))) (rdy_of_echoice cs) #
+      apply (rule exI[where x="WaitBlk (d + d2) (\<lambda>\<tau>. State (if \<tau> < d then p \<tau> else p2 (\<tau> - d))) (rdy_of_echoice cs) #
                                OutBlock ch (e (p2 d2)) # tr2'"])
       unfolding a apply auto
       subgoal by (rule e)
       using b by auto
     subgoal for i ch var p2 v tr2'
-      apply (rule exI[where x="WaitBlock d (\<lambda>\<tau>\<in>{0..d}. State (p \<tau>)) (rdy_of_echoice cs) # InBlock ch v # tr2'"])
+      apply (rule exI[where x="WaitBlk d (\<lambda>\<tau>. State (p \<tau>)) (rdy_of_echoice cs) # InBlock ch v # tr2'"])
       unfolding a apply auto apply (rule InterruptReceiveB2)
       by (auto simp add: InterruptS1)
     subgoal for d2 p2 i ch var p3 v tr2'
-      apply (rule exI[where x="WaitBlock (d + d2) (\<lambda>\<tau>\<in>{0..d+d2}. State (if \<tau> < d then p \<tau> else p2 (\<tau> - d))) (rdy_of_echoice cs) #
+      apply (rule exI[where x="WaitBlk (d + d2) (\<lambda>\<tau>. State (if \<tau> < d then p \<tau> else p2 (\<tau> - d))) (rdy_of_echoice cs) #
                                InBlock ch v # tr2'"])
       unfolding a apply auto
       subgoal by (rule f)
       using c by auto
     subgoal
-      apply (rule exI[where x="[WaitBlock d (\<lambda>\<tau>\<in>{0..d}. State (p \<tau>)) (rdy_of_echoice cs)]"])
+      apply (rule exI[where x="[WaitBlk d (\<lambda>\<tau>. State (p \<tau>)) (rdy_of_echoice cs)]"])
       unfolding a apply auto
       apply (rule InterruptB2)
       by (auto simp add: InterruptS1)
     subgoal for d2 p2
-      apply (rule exI[where x="[WaitBlock (d + d2) (\<lambda>\<tau>\<in>{0..d+d2}. State (if \<tau> < d then p \<tau> else p2 (\<tau> - d))) (rdy_of_echoice cs)]"])
+      apply (rule exI[where x="[WaitBlk (d + d2) (\<lambda>\<tau>. State (if \<tau> < d then p \<tau> else p2 (\<tau> - d))) (rdy_of_echoice cs)]"])
       unfolding a apply auto
       subgoal by (rule g)
       using d by auto
@@ -790,15 +791,15 @@ qed
 text \<open>Small-step generating WaitBlock can always be split into two smaller WaitBlocks\<close>
 
 lemma small_step_split:
-  "small_step p1 s1 (Some (WaitBlock t2 hist rdy)) p2 s2 \<Longrightarrow>
+  "small_step p1 s1 (Some (WaitBlk t2 hist rdy)) p2 s2 \<Longrightarrow>
    0 < t1 \<Longrightarrow> t1 < t2 \<Longrightarrow>
-   \<exists>p' s'. small_step p1 s1 (Some (WaitBlock t1 (\<lambda>\<tau>\<in>{0..t1}. hist \<tau>) rdy)) p' s' \<and>
-           small_step p' s' (Some (WaitBlock (t2 - t1) (\<lambda>\<tau>\<in>{0..t2-t1}. hist (\<tau> + t1)) rdy)) p2 s2"
-proof (induct p1 s1 "Some (WaitBlock t2 hist rdy)" p2 s2 rule: small_step.induct)
+   \<exists>p' s'. small_step p1 s1 (Some (WaitBlk t1 hist rdy)) p' s' \<and>
+           small_step p' s' (Some (WaitBlk (t2 - t1) (\<lambda>\<tau>. hist (\<tau> + t1)) rdy)) p2 s2"
+proof (induct p1 s1 "Some (WaitBlk t2 hist rdy)" p2 s2 rule: small_step.induct)
   case (seqS1 c1 s c1' s2 c2)
   obtain p' s' where a:
-    "small_step c1 s (Some (WaitBlock t1 (restrict hist {0..t1}) rdy)) p' s'"
-    "small_step p' s' (Some (WaitBlock (t2 - t1) (\<lambda>\<tau>\<in>{0..t2 - t1}. hist (\<tau> + t1)) rdy)) c1' s2"
+    "small_step c1 s (Some (WaitBlk t1 hist rdy)) p' s'"
+    "small_step p' s' (Some (WaitBlk (t2 - t1) (\<lambda>\<tau>. hist (\<tau> + t1)) rdy)) c1' s2"
     using seqS1 by auto
   show ?case
     apply (rule exI[where x="p'; c2"]) apply (rule exI[where x=s'])
@@ -806,131 +807,171 @@ proof (induct p1 s1 "Some (WaitBlock t2 hist rdy)" p2 s2 rule: small_step.induct
      apply (rule small_step.seqS1[OF a(1)])
     by (rule small_step.seqS1[OF a(2)])
 next
-  case (waitS1 d s)
-  have a: "restrict hist {0..t1} = (\<lambda>\<tau>\<in>{0..t1}. State s)"
-    unfolding waitS1(3)[symmetric] using waitS1(5,6) by auto
-  have b: "(\<lambda>\<tau>\<in>{0..t2-t1}. hist (\<tau> + t1)) = (\<lambda>\<tau>\<in>{0..t2-t1}. State s)"
-    unfolding waitS1(3)[symmetric] using waitS1(5,6) by auto
-  have c: "d - t2 = (d - t1) - (t2 - t1)" by auto
+  case (waitS1 d1 d s)
+  have a: "d1 = t2" "restrict hist {0..t2} = (\<lambda>\<tau>\<in>{0..t2}. State s)" "rdy = ({}, {})"
+    using waitS1(3) unfolding WaitBlk_def by auto
+  have b: "restrict hist {0..t1} = (\<lambda>\<tau>\<in>{0..t1}. State s)"
+    apply (rule ext)
+    using restrict_cong_to_eq[OF a(2)] using \<open>t1 < t2\<close> by auto
+  have c: "(\<lambda>\<tau>\<in>{0..t2-t1}. hist (\<tau> + t1)) = (\<lambda>\<tau>\<in>{0..t2-t1}. State s)"
+    apply (rule ext)
+    using restrict_cong_to_eq[OF a(2)] using \<open>t1 > 0\<close> by auto 
+  have d: "d - d1 = (d - t1) - (t2 - t1)"
+    by (auto simp add: a(1)) 
   show ?case
     apply (rule exI[where x="Wait (d - t1)"]) apply (rule exI[where x=s])
-    unfolding a b waitS1(4)[symmetric] apply auto
+    unfolding WaitBlk_def apply auto
     subgoal
-      apply (rule small_step.waitS1) using waitS1 by auto
+      unfolding b WaitBlk_def[symmetric] a(3)
+      apply (rule small_step.waitS1) using waitS1 \<open>d1 = t2\<close> by auto
     subgoal
-      unfolding c apply (rule small_step.waitS1) using waitS1 by auto
+      unfolding c WaitBlk_def[symmetric] a(3) d
+      apply (rule small_step.waitS1) using waitS1 \<open>d1 = t2\<close> by auto
     done
 next
-  case (waitS2 s)
-  have a: "restrict hist {0..t1} = (\<lambda>\<tau>\<in>{0..t1}. State s)"
-    unfolding waitS2(2)[symmetric] using waitS2(4,5) by auto
-  have b: "(\<lambda>\<tau>\<in>{0..t2-t1}. hist (\<tau> + t1)) = (\<lambda>\<tau>\<in>{0..t2-t1}. State s)"
-    unfolding waitS2(2)[symmetric] using waitS2(4,5) by auto
+  case (waitS2 d s)
+  have a: "d = t2" "restrict hist {0..t2} = (\<lambda>\<tau>\<in>{0..t2}. State s)" "rdy = ({}, {})"
+    using waitS2(2) unfolding WaitBlk_def by auto
+  have b: "restrict hist {0..t1} = (\<lambda>\<tau>\<in>{0..t1}. State s)"
+    apply (rule ext)
+    using restrict_cong_to_eq[OF a(2)] using \<open>t1 < t2\<close> by auto
+  have c: "(\<lambda>\<tau>\<in>{0..t2-t1}. hist (\<tau> + t1)) = (\<lambda>\<tau>\<in>{0..t2-t1}. State s)"
+    apply (rule ext)
+    using restrict_cong_to_eq[OF a(2)] using \<open>t1 > 0\<close> by auto 
   show ?case
-    apply (rule exI[where x="Wait (t2 - t1)"])
-    apply (rule exI[where x=s])
-    unfolding a b waitS2(3)[symmetric] apply auto
+    apply (rule exI[where x="Wait (t2 - t1)"]) apply (rule exI[where x=s])
+    unfolding WaitBlk_def apply auto
     subgoal
+      unfolding b WaitBlk_def[symmetric] a(1,3)
       apply (rule small_step.waitS1) using waitS2 by auto
     subgoal
+      unfolding c WaitBlk_def[symmetric] a(3)
       apply (rule small_step.waitS2) using waitS2 by auto
     done
 next
-  case (sendS2 ch e s)
-  have a: "restrict hist {0..t1} = (\<lambda>\<tau>\<in>{0..t1}. State s)"
-    unfolding sendS2(2)[symmetric] using sendS2(4,5) by auto
-  have b: "(\<lambda>\<tau>\<in>{0..t2-t1}. hist (\<tau> + t1)) = (\<lambda>\<tau>\<in>{0..t2-t1}. State s)"
-    unfolding sendS2(2)[symmetric] using sendS2(4,5) by auto
+  case (sendS2 d ch e s)
+  have a: "d = t2" "restrict hist {0..t2} = (\<lambda>\<tau>\<in>{0..t2}. State s)" "rdy = ({ch}, {})"
+    using sendS2(2) unfolding WaitBlk_def by auto
+  have b: "restrict hist {0..t1} = (\<lambda>\<tau>\<in>{0..t1}. State s)"
+    apply (rule ext)
+    using restrict_cong_to_eq[OF a(2)] using \<open>t1 < t2\<close> by auto
+  have c: "(\<lambda>\<tau>\<in>{0..t2-t1}. hist (\<tau> + t1)) = (\<lambda>\<tau>\<in>{0..t2-t1}. State s)"
+    apply (rule ext)
+    using restrict_cong_to_eq[OF a(2)] using \<open>t1 > 0\<close> by auto 
   show ?case
     apply (rule exI[where x="Cm (ch[!]e)"])
     apply (rule exI[where x=s])
-    unfolding a b sendS2(3)[symmetric] apply auto
+    unfolding WaitBlk_def apply auto
     subgoal
+      unfolding b WaitBlk_def[symmetric] a(1,3)
       apply (rule small_step.sendS2) using sendS2 by auto
     subgoal
+      unfolding c WaitBlk_def[symmetric] a(3)
       apply (rule small_step.sendS2) using sendS2 by auto
     done
 next
-  case (receiveS2 ch var s)
-  have a: "restrict hist {0..t1} = (\<lambda>\<tau>\<in>{0..t1}. State s)"
-    unfolding receiveS2(2)[symmetric] using receiveS2(4,5) by auto
-  have b: "(\<lambda>\<tau>\<in>{0..t2-t1}. hist (\<tau> + t1)) = (\<lambda>\<tau>\<in>{0..t2-t1}. State s)"
-    unfolding receiveS2(2)[symmetric] using receiveS2(4,5) by auto
+  case (receiveS2 d ch var s)
+  have a: "d = t2" "restrict hist {0..t2} = (\<lambda>\<tau>\<in>{0..t2}. State s)" "rdy = ({}, {ch})"
+    using receiveS2(2) unfolding WaitBlk_def by auto
+  have b: "restrict hist {0..t1} = (\<lambda>\<tau>\<in>{0..t1}. State s)"
+    apply (rule ext)
+    using restrict_cong_to_eq[OF a(2)] using \<open>t1 < t2\<close> by auto
+  have c: "(\<lambda>\<tau>\<in>{0..t2-t1}. hist (\<tau> + t1)) = (\<lambda>\<tau>\<in>{0..t2-t1}. State s)"
+    apply (rule ext)
+    using restrict_cong_to_eq[OF a(2)] using \<open>t1 > 0\<close> by auto 
   show ?case
     apply (rule exI[where x="Cm (ch[?]var)"])
     apply (rule exI[where x=s])
-    unfolding a b receiveS2(3)[symmetric] apply auto
+    unfolding WaitBlk_def apply auto
     subgoal
+      unfolding b WaitBlk_def[symmetric] a(1,3)
       apply (rule small_step.receiveS2) using receiveS2 by auto
     subgoal
+      unfolding c WaitBlk_def[symmetric] a(3)
       apply (rule small_step.receiveS2) using receiveS2 by auto
     done
 next
-  case (EChoiceS1 cs s)
-  have a: "restrict hist {0..t1} = (\<lambda>\<tau>\<in>{0..t1}. State s)"
-    unfolding EChoiceS1(2)[symmetric] using EChoiceS1(4,5) by auto
-  have b: "(\<lambda>\<tau>\<in>{0..t2-t1}. hist (\<tau> + t1)) = (\<lambda>\<tau>\<in>{0..t2-t1}. State s)"
-    unfolding EChoiceS1(2)[symmetric] using EChoiceS1(4,5) by auto
+  case (EChoiceS1 d cs s)
+  have a: "d = t2" "restrict hist {0..t2} = (\<lambda>\<tau>\<in>{0..t2}. State s)" "rdy = rdy_of_echoice cs"
+    using EChoiceS1(2) unfolding WaitBlk_def by auto
+  have b: "restrict hist {0..t1} = (\<lambda>\<tau>\<in>{0..t1}. State s)"
+    apply (rule ext)
+    using restrict_cong_to_eq[OF a(2)] using \<open>t1 < t2\<close> by auto
+  have c: "(\<lambda>\<tau>\<in>{0..t2-t1}. hist (\<tau> + t1)) = (\<lambda>\<tau>\<in>{0..t2-t1}. State s)"
+    apply (rule ext)
+    using restrict_cong_to_eq[OF a(2)] using \<open>t1 > 0\<close> by auto 
   show ?case
     apply (rule exI[where x="EChoice cs"])
     apply (rule exI[where x=s])
-    unfolding a b EChoiceS1(3)[symmetric] apply auto
+    unfolding WaitBlk_def apply auto
     subgoal
+      unfolding b WaitBlk_def[symmetric] a(1,3)
       apply (rule small_step.EChoiceS1) using EChoiceS1 by auto
     subgoal
+      unfolding c WaitBlk_def[symmetric] a(3)
       apply (rule small_step.EChoiceS1) using EChoiceS1 by auto
     done
 next
-  case (ContS1 ode p b s)
-  have a: "restrict hist {0..t1} = (\<lambda>\<tau>\<in>{0..t1}. State (p \<tau>))"
-    unfolding ContS1(5)[symmetric] using ContS1(7,8) by auto
-  have b: "(\<lambda>\<tau>\<in>{0..t2 - t1}. hist (\<tau> + t1)) = (\<lambda>\<tau>\<in>{0..t2-t1}. State (p (\<tau> + t1)))"
-    unfolding ContS1(5)[symmetric] using ContS1(7,8) by auto
-  have c: "p t2 = (\<lambda>t. p (t + t1)) (t2 - t1)"
+  case (ContS1 d ode p b s)
+  have a: "d = t2" "restrict hist {0..t2} = (\<lambda>\<tau>\<in>{0..t2}. State (p \<tau>))" "rdy = ({}, {})"
+    using ContS1(5) unfolding WaitBlk_def by auto
+  have b: "restrict hist {0..t1} = (\<lambda>\<tau>\<in>{0..t1}. State (p \<tau>))"
+    apply (rule ext)
+    using restrict_cong_to_eq[OF a(2)] using \<open>t1 < t2\<close> by auto
+  have c: "(\<lambda>\<tau>\<in>{0..t2-t1}. hist (\<tau> + t1)) = (\<lambda>\<tau>\<in>{0..t2-t1}. State (p (\<tau> + t1)))"
+    apply (rule ext)
+    using restrict_cong_to_eq[OF a(2)] using \<open>t1 > 0\<close> by auto
+  have d: "p t2 = (\<lambda>t. p (t + t1)) (t2 - t1)"
     by auto
   show ?case
     apply (rule exI[where x="Cont ode b"])
     apply (rule exI[where x="p t1"])
-    unfolding a b ContS1(6)[symmetric] apply auto
+    unfolding WaitBlk_def apply auto
     subgoal
+      unfolding b WaitBlk_def[symmetric] a(3)
       apply (rule small_step.ContS1)
          apply (simp add: ContS1.prems(1))
-      using ContS1 ODEsol_split(1) apply auto[1]
-      using ContS1 apply auto[1]
-      by (simp add: ContS1.hyps(4))
+        apply (rule ODEsol_split(1)[OF ContS1(2)])
+      using ContS1 a(1) by auto
     subgoal
-      unfolding c apply (rule small_step.ContS1)
+      unfolding c WaitBlk_def[symmetric] a(1,3) d
+      apply (rule small_step.ContS1)
          apply (simp add: ContS1.prems(2))
-        apply (simp add: ContS1 ODEsol_split(2))
-      using ContS1 apply auto[1]
-      by simp
+        apply (rule ODEsol_split(2))
+      using a(1) ContS1(2) apply auto[1]
+      using ContS1 a(1) by auto
     done
 next
-  case (InterruptS1 ode p b s cs)
-  have a: "restrict hist {0..t1} = (\<lambda>\<tau>\<in>{0..t1}. State (p \<tau>))"
-    unfolding InterruptS1(5)[symmetric] using InterruptS1(7,8) by auto
-  have b: "(\<lambda>\<tau>\<in>{0..t2 - t1}. hist (\<tau> + t1)) = (\<lambda>\<tau>\<in>{0..t2-t1}. State (p (\<tau> + t1)))"
-    unfolding InterruptS1(5)[symmetric] using InterruptS1(7,8) by auto
-  have c: "p t2 = (\<lambda>t. p (t + t1)) (t2 - t1)"
+  case (InterruptS1 d ode p b s cs)
+  have a: "d = t2" "restrict hist {0..t2} = (\<lambda>\<tau>\<in>{0..t2}. State (p \<tau>))" "rdy = rdy_of_echoice cs"
+    using InterruptS1(5) unfolding WaitBlk_def by auto
+  have b: "restrict hist {0..t1} = (\<lambda>\<tau>\<in>{0..t1}. State (p \<tau>))"
+    apply (rule ext)
+    using restrict_cong_to_eq[OF a(2)] using \<open>t1 < t2\<close> by auto
+  have c: "(\<lambda>\<tau>\<in>{0..t2-t1}. hist (\<tau> + t1)) = (\<lambda>\<tau>\<in>{0..t2-t1}. State (p (\<tau> + t1)))"
+    apply (rule ext)
+    using restrict_cong_to_eq[OF a(2)] using \<open>t1 > 0\<close> by auto
+  have d: "p t2 = (\<lambda>t. p (t + t1)) (t2 - t1)"
     by auto
   show ?case
     apply (rule exI[where x="Interrupt ode b cs"])
     apply (rule exI[where x="p t1"])
-    unfolding a b InterruptS1(6)[symmetric] apply auto
+    unfolding WaitBlk_def apply auto
     subgoal
+      unfolding b WaitBlk_def[symmetric] a(3)
       apply (rule small_step.InterruptS1)
          apply (simp add: InterruptS1.prems(1))
-      using InterruptS1 ODEsol_split(1) apply auto[1]
-      using InterruptS1 apply auto[1]
-      by (simp add: InterruptS1.hyps(4))
+        apply (rule ODEsol_split(1)[OF InterruptS1(2)])
+      using InterruptS1 a(1) by auto
     subgoal
-      unfolding c apply (rule small_step.InterruptS1)
+      unfolding c WaitBlk_def[symmetric] a(1,3) d
+      apply (rule small_step.InterruptS1)
          apply (simp add: InterruptS1.prems(2))
-        apply (simp add: InterruptS1 ODEsol_split(2))
-      using InterruptS1 apply auto[1]
-      by simp
+        apply (rule ODEsol_split(2))
+      using a(1) InterruptS1(2) apply auto[1]
+      using InterruptS1 a(1) by auto
     done
-qed
+qed (auto simp add: WaitBlk_def)
 
 
 subsection \<open>Parallel case\<close>
@@ -945,11 +986,11 @@ inductive par_small_step :: "pproc \<Rightarrow> gstate \<Rightarrow> trace_bloc
   SingleS: "small_step p s1 ev p' s2 \<Longrightarrow> par_small_step (Single p) (State s1) ev (Single p') (State s2)"
 | ParDelayS:
     "compat_rdy rdy1 rdy2 \<Longrightarrow>
-     hist = (\<lambda>\<tau>\<in>{0..t}. ParState (hist1 \<tau>) (hist2 \<tau>)) \<Longrightarrow>
+     hist = (\<lambda>\<tau>. ParState (hist1 \<tau>) (hist2 \<tau>)) \<Longrightarrow>
      rdy = merge_rdy rdy1 rdy2 \<Longrightarrow>
-     par_small_step p1 s1 (Some (WaitBlock t hist1 rdy1)) p2 s2 \<Longrightarrow>
-     par_small_step p3 s3 (Some (WaitBlock t hist2 rdy2)) p4 s4 \<Longrightarrow>
-     par_small_step (Parallel p1 chs p3) (ParState s1 s3) (Some (WaitBlock t hist rdy)) (Parallel p2 chs p4) (ParState s2 s4)"
+     par_small_step p1 s1 (Some (WaitBlk t hist1 rdy1)) p2 s2 \<Longrightarrow>
+     par_small_step p3 s3 (Some (WaitBlk t hist2 rdy2)) p4 s4 \<Longrightarrow>
+     par_small_step (Parallel p1 chs p3) (ParState s1 s3) (Some (WaitBlk t hist rdy)) (Parallel p2 chs p4) (ParState s2 s4)"
 | ParTauS1:
     "wf_pair p3 s3 \<Longrightarrow>
      par_small_step p1 s1 None p2 s2 \<Longrightarrow>
@@ -1131,15 +1172,15 @@ qed
 text \<open>Analogous result to small_step_split for the parallel case\<close>
 
 lemma par_small_step_split:
-  "par_small_step p1 s1 (Some (WaitBlock t2 hist rdy)) p2 s2 \<Longrightarrow>
+  "par_small_step p1 s1 (Some (WaitBlk t2 hist rdy)) p2 s2 \<Longrightarrow>
    0 < t1 \<Longrightarrow> t1 < t2 \<Longrightarrow>
-   \<exists>p' s'. par_small_step p1 s1 (Some (WaitBlock t1 (\<lambda>\<tau>\<in>{0..t1}. hist \<tau>) rdy)) p' s' \<and>
-           par_small_step p' s' (Some (WaitBlock (t2 - t1) (\<lambda>\<tau>\<in>{0..t2-t1}. hist (\<tau> + t1)) rdy)) p2 s2"
-proof (induct p1 s1 "Some (WaitBlock t2 hist rdy)" p2 s2 arbitrary: hist rdy rule: par_small_step.induct)
+   \<exists>p' s'. par_small_step p1 s1 (Some (WaitBlk t1 hist rdy)) p' s' \<and>
+           par_small_step p' s' (Some (WaitBlk (t2 - t1) (\<lambda>\<tau>. hist (\<tau> + t1)) rdy)) p2 s2"
+proof (induct p1 s1 "Some (WaitBlk t2 hist rdy)" p2 s2 arbitrary: hist rdy rule: par_small_step.induct)
   case (SingleS p s1 p' s2)
   obtain pp ss where a:
-    "small_step p s1 (Some (WaitBlock t1 (restrict hist {0..t1}) rdy)) pp ss"
-    "small_step pp ss (Some (WaitBlock (t2 - t1) (\<lambda>\<tau>\<in>{0..t2 - t1}. hist (\<tau> + t1)) rdy)) p' s2"
+    "small_step p s1 (Some (WaitBlk t1 hist rdy)) pp ss"
+    "small_step pp ss (Some (WaitBlk (t2 - t1) (\<lambda>\<tau>. hist (\<tau> + t1)) rdy)) p' s2"
     using small_step_split[OF SingleS(1-3)] by auto
   show ?case
     apply (rule exI[where x="Single pp"])
@@ -1147,27 +1188,36 @@ proof (induct p1 s1 "Some (WaitBlock t2 hist rdy)" p2 s2 arbitrary: hist rdy rul
     apply auto apply (rule par_small_step.SingleS[OF a(1)])
     by (rule par_small_step.SingleS[OF a(2)])
 next
-  case (ParDelayS rdy1 rdy2 hist hist1 hist2 rdy p1 s1 p2 s2 p3 s3 p4 s4 chs)
-  obtain p1' s1' where a:
-    "par_small_step p1 s1 (Some (WaitBlock t1 (restrict hist1 {0..t1}) rdy1)) p1' s1'"
-    "par_small_step p1' s1' (Some (WaitBlock (t2 - t1) (\<lambda>\<tau>\<in>{0..t2 - t1}. hist1 (\<tau> + t1)) rdy1)) p2 s2"
-    using ParDelayS(5,8,9) by auto
-  obtain p3' s3' where b:
-    "par_small_step p3 s3 (Some (WaitBlock t1 (restrict hist2 {0..t1}) rdy2)) p3' s3'"
-    "par_small_step p3' s3' (Some (WaitBlock (t2 - t1) (\<lambda>\<tau>\<in>{0..t2 - t1}. hist2 (\<tau> + t1)) rdy2)) p4 s4"
-    using ParDelayS(7,8,9) by auto
+  case (ParDelayS rdy1 rdy2 hist' hist1 hist2 rdy' p1 s1 t p2 s2 p3 s3 p4 s4 chs)
+  have a: "t = t2" "restrict hist {0..t2} = restrict hist' {0..t2}" "rdy = rdy'"
+    using ParDelayS(8) unfolding WaitBlk_def by auto
+  have a2: "WaitBlk t1 hist rdy' = WaitBlk t1 hist' rdy'"
+    using restrict_cong_to_eq[OF a(2)] unfolding WaitBlk_def
+    apply auto apply (rule ext) using \<open>t1 < t2\<close> by auto
+  have a3: "WaitBlk (t2 - t1) (\<lambda>\<tau>. hist (\<tau> + t1)) rdy' = WaitBlk (t2 - t1) (\<lambda>\<tau>. hist' (\<tau> + t1)) rdy'"
+    using restrict_cong_to_eq[OF a(2)] unfolding WaitBlk_def
+    apply auto apply (rule ext) using \<open>t1 < t2\<close> \<open>0 < t1\<close> by auto
+  obtain p1' s1' where b:
+    "par_small_step p1 s1 (Some (WaitBlk t1 hist1 rdy1)) p1' s1'"
+    "par_small_step p1' s1' (Some (WaitBlk (t2 - t1) (\<lambda>\<tau>. hist1 (\<tau> + t1)) rdy1)) p2 s2"
+    using ParDelayS(5,9,10)[unfolded a(1)] by blast
+  obtain p3' s3' where c:
+    "par_small_step p3 s3 (Some (WaitBlk t1 hist2 rdy2)) p3' s3'"
+    "par_small_step p3' s3' (Some (WaitBlk (t2 - t1) (\<lambda>\<tau>. hist2 (\<tau> + t1)) rdy2)) p4 s4"
+    using ParDelayS(7,9,10)[unfolded a(1)] by blast
   show ?case
     apply (rule exI[where x="Parallel p1' chs p3'"])
     apply (rule exI[where x="ParState s1' s3'"])
     apply auto
     subgoal
-      apply (rule par_small_step.ParDelayS[OF ParDelayS(1) _ ParDelayS(3) a(1) b(1)])
-      using ParDelayS(2,8,9) by auto
+      unfolding a(3) a2
+      by (rule par_small_step.ParDelayS[OF ParDelayS(1-3) b(1) c(1)])
     subgoal
-      apply (rule par_small_step.ParDelayS[OF ParDelayS(1) _ ParDelayS(3) a(2) b(2)])
-      using ParDelayS(2,8,9) by auto
+      unfolding a(3) a3
+      apply (rule par_small_step.ParDelayS[OF ParDelayS(1) _ ParDelayS(3) b(2) c(2)])
+      using ParDelayS(2) by auto
     done
-qed  
+qed (auto simp add: WaitBlk_def)
 
 
 inductive is_skip :: "pproc \<Rightarrow> bool" where
@@ -1264,20 +1314,20 @@ next
   show ?case
     using b c d par_small_step_closure.intros(3) par_small_step_closure_trans by fastforce 
 next
-  case (combine_blocks_wait1 chs blks1 blks2 blks rdy1 rdy2 hist hist1 hist2 t rdy)
+  case (combine_blocks_wait1 chs blks1 blks2 blks rdy1 rdy2 hist hist1 hist2 rdy t)
   obtain p1' s1' p1'' s1'' where a:
     "par_small_step_tau_closure p1 s11 p1' s1'"
-    "par_small_step p1' s1' (Some (WaitBlock t hist1 rdy1)) p1'' s1''"
+    "par_small_step p1' s1' (Some (WaitBlk t hist1 rdy1)) p1'' s1''"
     "par_small_step_closure p1'' s1'' blks1 p3 s12"
     using par_small_step_closure_cons_to_tau[OF combine_blocks_wait1(6)] by auto
   obtain p2' s2' p2'' s2'' where b:
     "par_small_step_tau_closure p2 s21 p2' s2'"
-    "par_small_step p2' s2' (Some (WaitBlock t hist2 rdy2)) p2'' s2''"
+    "par_small_step p2' s2' (Some (WaitBlk t hist2 rdy2)) p2'' s2''"
     "par_small_step_closure p2'' s2'' blks2 p4 s22"
     using par_small_step_closure_cons_to_tau[OF combine_blocks_wait1(7)] by auto
   have c: "par_small_step_closure (Parallel p1 chs p2) (ParState s11 s21) [] (Parallel p1' chs p2') (ParState s1' s2')"
     by (rule par_small_step_closure_merge[OF a(1) b(1)])
-  have d: "par_small_step (Parallel p1' chs p2') (ParState s1' s2') (Some (WaitBlock t hist rdy))
+  have d: "par_small_step (Parallel p1' chs p2') (ParState s1' s2') (Some (WaitBlk t hist rdy))
            (Parallel p1'' chs p2'') (ParState s1'' s2'')"
     apply (rule ParDelayS)
     using combine_blocks_wait1 a(2) b(2) by auto
@@ -1289,21 +1339,21 @@ next
   case (combine_blocks_wait2 chs blks1 t2 t1 hist2 rdy2 blks2 blks rdy1 hist hist1 rdy)
   obtain p1' s1' p1'' s1'' where a:
     "par_small_step_tau_closure p1 s11 p1' s1'"
-    "par_small_step p1' s1' (Some (WaitBlock t1 hist1 rdy1)) p1'' s1''"
+    "par_small_step p1' s1' (Some (WaitBlk t1 hist1 rdy1)) p1'' s1''"
     "par_small_step_closure p1'' s1'' blks1 p3 s12"
     using par_small_step_closure_cons_to_tau[OF combine_blocks_wait2(8)] by auto
   obtain p2' s2' p2'' s2'' where b:
     "par_small_step_tau_closure p2 s21 p2' s2'"
-    "par_small_step p2' s2' (Some (WaitBlock t2 hist2 rdy2)) p2'' s2''"
+    "par_small_step p2' s2' (Some (WaitBlk t2 hist2 rdy2)) p2'' s2''"
     "par_small_step_closure p2'' s2'' blks2 p4 s22"
     using par_small_step_closure_cons_to_tau[OF combine_blocks_wait2(9)] by auto
   have c: "par_small_step_closure (Parallel p1 chs p2) (ParState s11 s21) [] (Parallel p1' chs p2') (ParState s1' s2')"
     by (rule par_small_step_closure_merge[OF a(1) b(1)])
   obtain p2a s2a where d:
-    "par_small_step p2' s2' (Some (WaitBlock t1 (\<lambda>\<tau>\<in>{0..t1}. hist2 \<tau>) rdy2)) p2a s2a"
-    "par_small_step p2a s2a (Some (WaitBlock (t2 - t1) (\<lambda>\<tau>\<in>{0..t2-t1}. hist2 (\<tau> + t1)) rdy2)) p2'' s2''"
+    "par_small_step p2' s2' (Some (WaitBlk t1 hist2 rdy2)) p2a s2a"
+    "par_small_step p2a s2a (Some (WaitBlk (t2 - t1) (\<lambda>\<tau>. hist2 (\<tau> + t1)) rdy2)) p2'' s2''"
     using par_small_step_split[OF b(2) combine_blocks_wait2(4,3)] by auto
-  have e: "par_small_step (Parallel p1' chs p2') (ParState s1' s2') (Some (WaitBlock t1 hist rdy))
+  have e: "par_small_step (Parallel p1' chs p2') (ParState s1' s2') (Some (WaitBlk t1 hist rdy))
                           (Parallel p1'' chs p2a) (ParState s1'' s2a)"
     apply (rule ParDelayS)
     using combine_blocks_wait2(2,5,6) a(2) d(1) by auto
@@ -1317,21 +1367,21 @@ next
   case (combine_blocks_wait3 chs t1 t2 hist1 rdy1 blks1 blks2 blks rdy2 hist hist2 rdy)
   obtain p1' s1' p1'' s1'' where a:
     "par_small_step_tau_closure p1 s11 p1' s1'"
-    "par_small_step p1' s1' (Some (WaitBlock t1 hist1 rdy1)) p1'' s1''"
+    "par_small_step p1' s1' (Some (WaitBlk t1 hist1 rdy1)) p1'' s1''"
     "par_small_step_closure p1'' s1'' blks1 p3 s12"
     using par_small_step_closure_cons_to_tau[OF combine_blocks_wait3(8)] by auto
   obtain p2' s2' p2'' s2'' where b:
     "par_small_step_tau_closure p2 s21 p2' s2'"
-    "par_small_step p2' s2' (Some (WaitBlock t2 hist2 rdy2)) p2'' s2''"
+    "par_small_step p2' s2' (Some (WaitBlk t2 hist2 rdy2)) p2'' s2''"
     "par_small_step_closure p2'' s2'' blks2 p4 s22"
     using par_small_step_closure_cons_to_tau[OF combine_blocks_wait3(9)] by auto
   have c: "par_small_step_closure (Parallel p1 chs p2) (ParState s11 s21) [] (Parallel p1' chs p2') (ParState s1' s2')"
     by (rule par_small_step_closure_merge[OF a(1) b(1)])
   obtain p1a s1a where d:
-    "par_small_step p1' s1' (Some (WaitBlock t2 (\<lambda>\<tau>\<in>{0..t2}. hist1 \<tau>) rdy1)) p1a s1a"
-    "par_small_step p1a s1a (Some (WaitBlock (t1 - t2) (\<lambda>\<tau>\<in>{0..t1-t2}. hist1 (\<tau> + t2)) rdy1)) p1'' s1''"
+    "par_small_step p1' s1' (Some (WaitBlk t2 hist1 rdy1)) p1a s1a"
+    "par_small_step p1a s1a (Some (WaitBlk (t1 - t2) (\<lambda>\<tau>. hist1 (\<tau> + t2)) rdy1)) p1'' s1''"
     using par_small_step_split[OF a(2) combine_blocks_wait3(4,3)] by auto
-  have e: "par_small_step (Parallel p1' chs p2') (ParState s1' s2') (Some (WaitBlock t2 hist rdy))
+  have e: "par_small_step (Parallel p1' chs p2') (ParState s1' s2') (Some (WaitBlk t2 hist rdy))
                           (Parallel p1a chs p2'') (ParState s1a s2'')"
     apply (rule ParDelayS)
     using combine_blocks_wait3(2,5,6) b(2) d(1) by auto
@@ -1432,11 +1482,11 @@ next
   then show ?case
     by (meson combine_blocks.combine_blocks_unpair2 reduce_trace_cons)
 next
-  case (combine_blocks_wait1 comms blks1 blks2 blks rdy1 rdy2 hist hist1 hist2 t rdy)
+  case (combine_blocks_wait1 comms blks1 blks2 blks rdy1 rdy2 hist hist1 hist2 rdy t)
   obtain tr'' where a: "reduce_trace blks tr''" "combine_blocks comms tr2' blks2 tr''"
     using combine_blocks_wait1(1,6) by auto
   show ?case
-    apply (rule exI[where x="WaitBlock t hist rdy # tr''"])
+    apply (rule exI[where x="WaitBlk t hist rdy # tr''"])
     apply auto
     apply (rule reduce_trace_cons[OF a(1)])
     by (rule combine_blocks.combine_blocks_wait1[OF a(2) combine_blocks_wait1(3-5)])
@@ -1444,10 +1494,10 @@ next
   case (combine_blocks_wait2 comms blks1 t2 t1 hist2 rdy2 blks2 blks rdy1 hist hist1 rdy)
   obtain tr'' where a:
     "reduce_trace blks tr''"
-    "combine_blocks comms tr2' (WaitBlock (t2 - t1) (\<lambda>\<tau>\<in>{0..t2 - t1}. hist2 (\<tau> + t1)) rdy2 # blks2) tr''"
+    "combine_blocks comms tr2' (WaitBlk (t2 - t1) (\<lambda>\<tau>. hist2 (\<tau> + t1)) rdy2 # blks2) tr''"
     using combine_blocks_wait2(8)[OF combine_blocks_wait2(1)] by auto
   show ?case
-    apply (rule exI[where x="WaitBlock t1 hist rdy # tr''"])
+    apply (rule exI[where x="WaitBlk t1 hist rdy # tr''"])
     apply auto
     apply (rule reduce_trace_cons[OF a(1)])
     apply (rule combine_blocks.combine_blocks_wait2)
@@ -1455,10 +1505,10 @@ next
 next
   case (combine_blocks_wait3 comms t1 t2 hist1 rdy1 blks1 blks2 blks rdy2 hist hist2 rdy)
   obtain tr' where a:
-    "reduce_trace blks tr'" "combine_blocks comms (WaitBlock (t1 - t2) (\<lambda>\<tau>\<in>{0..t1-t2}. hist1 (\<tau> + t2)) rdy1 # tr2') blks2 tr'"
+    "reduce_trace blks tr'" "combine_blocks comms (WaitBlk (t1 - t2) (\<lambda>\<tau>. hist1 (\<tau> + t2)) rdy1 # tr2') blks2 tr'"
     using combine_blocks_wait3(2,8) by auto
   show ?case
-    apply (rule exI[where x="WaitBlock t2 hist rdy # tr'"])
+    apply (rule exI[where x="WaitBlk t2 hist rdy # tr'"])
     apply auto
     apply (rule reduce_trace_cons[OF a(1)])
     apply (rule combine_blocks.combine_blocks_wait3)
@@ -1486,11 +1536,11 @@ next
   then show ?case
     by (meson combine_blocks.combine_blocks_unpair2 reduce_trace_cons)
 next
-  case (combine_blocks_wait1 comms blks1 blks2 blks rdy1 rdy2 hist hist1 hist2 t rdy)
+  case (combine_blocks_wait1 comms blks1 blks2 blks rdy1 rdy2 hist hist1 hist2 rdy t)
   obtain tr'' where a: "reduce_trace blks tr''" "combine_blocks comms blks1 tr2' tr''"
     using combine_blocks_wait1(1,6) by auto
   show ?case
-    apply (rule exI[where x="WaitBlock t hist rdy # tr''"])
+    apply (rule exI[where x="WaitBlk t hist rdy # tr''"])
     apply auto
     apply (rule reduce_trace_cons[OF a(1)])
     by (rule combine_blocks.combine_blocks_wait1[OF a(2) combine_blocks_wait1(3-5)])
@@ -1498,10 +1548,10 @@ next
   case (combine_blocks_wait2 comms blks1 t2 t1 hist2 rdy2 blks2 blks rdy1 hist hist1 rdy)
   obtain tr' where a:
     "reduce_trace blks tr'"
-    "combine_blocks comms blks1 (WaitBlock (t2 - t1) (\<lambda>\<tau>\<in>{0..t2-t1}. hist2 (\<tau> + t1)) rdy2 # tr2') tr'"
+    "combine_blocks comms blks1 (WaitBlk (t2 - t1) (\<lambda>\<tau>. hist2 (\<tau> + t1)) rdy2 # tr2') tr'"
     using combine_blocks_wait2(2,8) by auto
   show ?case
-    apply (rule exI[where x="WaitBlock t1 hist rdy # tr'"])
+    apply (rule exI[where x="WaitBlk t1 hist rdy # tr'"])
     apply auto
     apply (rule reduce_trace_cons[OF a(1)])
     apply (rule combine_blocks.combine_blocks_wait2)
@@ -1510,10 +1560,10 @@ next
   case (combine_blocks_wait3 comms t1 t2 hist1 rdy1 blks1 blks2 blks rdy2 hist hist2 rdy)
   obtain tr'' where a:
     "reduce_trace blks tr''"
-    "combine_blocks comms (WaitBlock (t1 - t2) (\<lambda>\<tau>\<in>{0..t1-t2}. hist1 (\<tau> + t2)) rdy1 # blks1) tr2' tr''"
+    "combine_blocks comms (WaitBlk (t1 - t2) (\<lambda>\<tau>. hist1 (\<tau> + t2)) rdy1 # blks1) tr2' tr''"
     using combine_blocks_wait3(8)[OF combine_blocks_wait3(1)] by auto
   show ?case
-    apply (rule exI[where x="WaitBlock t2 hist rdy # tr''"])
+    apply (rule exI[where x="WaitBlk t2 hist rdy # tr''"])
     apply auto
     apply (rule reduce_trace_cons[OF a(1)])
     apply (rule combine_blocks.combine_blocks_wait3)
@@ -1522,53 +1572,61 @@ qed
 
 
 lemma combine_blocks_merge_left:
-  "combine_blocks chs (WaitBlock d1 (restrict p1 {0..d1}) rdy # WaitBlock d2 (restrict p2 {0..d2}) rdy # tr') tr2 tr \<Longrightarrow>
+  "combine_blocks chs (WaitBlk d1 p1 rdy # WaitBlk d2 p2 rdy # tr') tr2 tr \<Longrightarrow>
    p1 d1 = p2 0 \<Longrightarrow>
    d1 > 0 \<Longrightarrow> d2 > 0 \<Longrightarrow>
    \<exists>tr''. reduce_trace tr tr'' \<and>
-   combine_blocks chs (WaitBlock (d1 + d2) (\<lambda>\<tau>\<in>{0..d1+d2}. if \<tau> < d1 then p1 \<tau> else p2 (\<tau> - d1)) rdy # tr') tr2 tr''"
-proof (induct chs "WaitBlock d1 (restrict p1 {0..d1}) rdy # WaitBlock d2 (restrict p2 {0..d2}) rdy # tr'" tr2 tr
+   combine_blocks chs (WaitBlk (d1 + d2) (\<lambda>\<tau>. if \<tau> < d1 then p1 \<tau> else p2 (\<tau> - d1)) rdy # tr') tr2 tr''"
+proof (induct chs "WaitBlk d1 p1 rdy # WaitBlk d2 p2 rdy # tr'" tr2 tr
        arbitrary: d1 p1 rule: combine_blocks.induct)
   case (combine_blocks_unpair2 ch comms blks2 blks ch_type v)
   then show ?case
     using combine_blocks.combine_blocks_unpair2 reduce_trace_cons by blast
 next
-  case (combine_blocks_wait1 chs blks2 blks rdy2 hist hist2 t rdy')
-  have a: "(\<lambda>\<tau>\<in>{0..d2}. if 0 \<le> \<tau> + t \<and> \<tau> \<le> d2 then if \<tau> + t < t then p1 (\<tau> + t) else p2 (\<tau> + t - t) else undefined) =
-           (\<lambda>\<tau>\<in>{0..d2}. p2 \<tau>)" if "t > 0"
+  case (combine_blocks_wait1 chs blks2 blks rdy1 rdy2 hist hist1 hist2 rdy' t)
+  have a: "t = d1" "restrict hist1 {0..t} = restrict p1 {0..t}" "rdy = rdy1"
+    using combine_blocks_wait1(6) unfolding WaitBlk_def by auto
+  have b: "(\<lambda>\<tau>\<in>{0..d2}. if \<tau> < 0 then p1 (\<tau> + t) else p2 (\<tau> + t - d1)) = (\<lambda>\<tau>\<in>{0..d2}. p2 \<tau>)"
     apply (rule restrict_ext)
-    using combine_blocks_wait1 that by auto
+    by (auto simp add: a(1))
+  have c: "WaitBlk t hist rdy' = WaitBlk t (\<lambda>\<tau>. ParState (if \<tau> < d1 then p1 \<tau> else p2 (\<tau> - d1)) (hist2 \<tau>)) rdy'"
+    unfolding WaitBlk_def apply (auto simp add: combine_blocks_wait1(4))
+    apply (rule ext)
+    using restrict_combine_cong[OF a(2)]
+    by (auto simp add: a combine_blocks_wait1(7))
   show ?case
-    apply (rule exI[where x="WaitBlock t hist rdy' # blks"])
-    apply auto
+    apply (rule exI[where x="WaitBlk t hist rdy' # blks"])
+    apply auto unfolding c
     apply (rule combine_blocks_wait3)
-    subgoal apply (auto simp add: combine_blocks_wait1)
-      unfolding a
-      by (simp add: a combine_blocks_wait1.hyps(1) combine_blocks_wait1.prems(2))
-    using combine_blocks_wait1 by auto
+    subgoal
+      apply (auto simp add: a(1) WaitBlk_def b)
+      using combine_blocks_wait1(1)[unfolded WaitBlk_def] by auto
+    using combine_blocks_wait1 a by auto
 next
-  case (combine_blocks_wait2 comms t2 t1 hist2 rdy2 blks2 blks hist rdy')
+  case (combine_blocks_wait2 comms t2 t1 hist2 rdy2 blks2 blks rdy1 hist hist1 rdy')
+  have pre: "d1 = t1" "restrict hist1 {0..t1} = restrict p1 {0..t1}" "rdy1 = rdy"
+    using combine_blocks_wait2(8) unfolding WaitBlk_def by auto
   have a: ?case if "t1 + d2 = t2"
   proof -
     have a1: "t2 - t1 = d2"
       using that by auto
     obtain blks' where a2:
-      "blks = WaitBlock d2 (\<lambda>t\<in>{0..d2}. ParState (restrict p2 {0..d2} t) ((\<lambda>\<tau>\<in>{0..d2}. hist2 (\<tau> + t1)) t)) rdy' # blks'"
+      "blks = WaitBlk d2 (\<lambda>t. ParState (p2 t) (hist2 (t + t1))) rdy' # blks'"
       "combine_blocks comms tr' blks2 blks'"
       using combine_blocks_waitE2[OF combine_blocks_wait2(1)[unfolded a1]]
-            combine_blocks_wait2(3,7) by auto
+            combine_blocks_wait2(3,7) pre(3) by auto
     show ?thesis
       unfolding a2(1)
-      apply (rule exI[where x="WaitBlock (t1 + d2) (\<lambda>\<tau>\<in>{0..t1+d2}. ParState (if \<tau> < t1 then p1 \<tau> else p2 (\<tau> - t1)) (hist2 \<tau>)) rdy' # blks'"])
+      apply (rule exI[where x="WaitBlk (t1 + d2) (\<lambda>\<tau>. ParState (if \<tau> < t1 then p1 \<tau> else p2 (\<tau> - t1)) (hist2 \<tau>)) rdy' # blks'"])
       apply auto
       subgoal
         unfolding combine_blocks_wait2(6)
         apply (rule reduce_trace_merge')
-        using combine_blocks_wait2(8-10) by auto
+        using combine_blocks_wait2(9-11) restrict_cong_to_eq[OF pre(2)] pre(1) by auto
       subgoal
-        unfolding that
+        unfolding pre(1) that
         apply (rule combine_blocks.combine_blocks_wait1)
-        using combine_blocks_wait2(3,7) a2(2) by auto
+        using combine_blocks_wait2(3,7) a2(2) pre(3) by auto
       done
   qed
   have b: ?case if "t1 + d2 < t2"
@@ -1576,171 +1634,181 @@ next
     have b1: "d2 < t2 - t1"
       using that by auto
     obtain blks' where b2:
-      "blks = WaitBlock d2 (\<lambda>t\<in>{0..d2}. ParState (restrict p2 {0..d2} t) ((\<lambda>\<tau>\<in>{0..t2-t1}. hist2 (\<tau> + t1)) t)) rdy' # blks'"
-      "combine_blocks comms tr' (WaitBlock (t2-t1-d2) (\<lambda>t\<in>{0..t2-t1-d2}. (\<lambda>\<tau>\<in>{0..t2-t1}. hist2 (\<tau> + t1)) (t + d2)) rdy2 # blks2) blks'"
-      using combine_blocks_waitE3[OF combine_blocks_wait2(1) b1 combine_blocks_wait2(3)]
-            combine_blocks_wait2(7) by auto
-    have b3: "t2 - t1 - d2 = t2 - (t1 + d2)"
-      by auto
-    have b4:
-      "(\<lambda>t\<in>{0..t2-t1-d2}. (\<lambda>\<tau>\<in>{0..t2-t1}. hist2 (\<tau> + t1)) (t + d2)) = (\<lambda>\<tau>\<in>{0..t2-(t1+d2)}. hist2 (\<tau> + (t1 + d2)))"
-      unfolding b3 apply (rule restrict_ext)
-      apply auto
-       apply (metis add.assoc add.commute)
-      using combine_blocks_wait2.prems(3) by auto
+      "blks = WaitBlk d2 (\<lambda>t. ParState (p2 t) (hist2 (t + t1))) rdy' # blks'"
+      "combine_blocks comms tr' (WaitBlk (t2 - t1 - d2) (\<lambda>t. hist2 (t + d2 + t1)) rdy2 # blks2) blks'"
+      using combine_blocks_waitE3[OF combine_blocks_wait2(1,11) b1]
+            combine_blocks_wait2(3,7) unfolding pre(3) by auto
+    have b3: "WaitBlk (t2 - t1 - d2) (\<lambda>t. hist2 (t + d2 + t1)) rdy2 = WaitBlk (t2 - (t1 + d2)) (\<lambda>\<tau>. hist2 (\<tau> + (t1 + d2))) rdy2"
+      apply (auto simp add: WaitBlk_def)
+      apply (rule ext) by (auto simp add: add.commute add.left_commute)
     show ?thesis
       unfolding b2(1)
-      apply (rule exI[where x="WaitBlock (t1 + d2) (\<lambda>\<tau>\<in>{0..t1+d2}. ParState (if \<tau> < t1 then p1 \<tau> else p2 (\<tau> - t1)) (hist2 \<tau>)) rdy' # blks'"])
+      apply (rule exI[where x="WaitBlk (t1 + d2) (\<lambda>\<tau>. ParState (if \<tau> < t1 then p1 \<tau> else p2 (\<tau> - t1)) (hist2 \<tau>)) rdy' # blks'"])
       apply auto
       subgoal
         unfolding combine_blocks_wait2(6)
         apply (rule reduce_trace_merge')
-        using combine_blocks_wait2(8-10) b1 by auto
+        using combine_blocks_wait2(9-11) restrict_cong_to_eq[OF pre(2)] b1 pre(1) by auto
       subgoal
+        unfolding pre(1)
         apply (rule combine_blocks.combine_blocks_wait2)
-        using combine_blocks_wait2(3,7-10) that b2(2)
-        unfolding b4 unfolding b3 by auto
+        using combine_blocks_wait2(3,7-11) that b2(2)
+        unfolding b3 pre by auto
       done
   qed
   have c: ?case if "t1 + d2 > t2"
   proof -
-    have c1: "t2 - t1 < d2"
-      using that by auto
+    have c1: "0 < t2 - t1" "t2 - t1 < d2"
+      using that combine_blocks_wait2(4) by auto
     obtain blks' where c2:
-      "blks = WaitBlock (t2 - t1) (\<lambda>t\<in>{0..t2-t1}. ParState (restrict p2 {0..d2} t) ((\<lambda>\<tau>\<in>{0..t2-t1}. hist2 (\<tau> + t1)) t)) rdy' # blks'"
-      "combine_blocks comms (WaitBlock (d2 - (t2 - t1)) (\<lambda>t\<in>{0..d2-(t2-t1)}. restrict p2 {0..d2} (t + (t2 - t1))) rdy # tr') blks2 blks'"
-      using combine_blocks_waitE4[OF combine_blocks_wait2(1) c1 combine_blocks_wait2(3)]
-            combine_blocks_wait2(7) by auto
-    have c3: "WaitBlock t2 (\<lambda>\<tau>\<in>{0..t2}. ParState (if \<tau> < t1 then p1 \<tau> else p2 (\<tau> - t1)) (hist2 \<tau>)) rdy' =
-              WaitBlock (t1 + (t2 - t1)) (\<lambda>\<tau>\<in>{0..t1+(t2-t1)}. ParState (if \<tau> < t1 then p1 \<tau> else p2 (\<tau> - t1)) (hist2 \<tau>)) rdy'"
+      "blks = WaitBlk (t2 - t1) (\<lambda>t. ParState (p2 t) (hist2 (t + t1))) rdy' # blks'"
+      "combine_blocks comms (WaitBlk (d2 - (t2 - t1)) (\<lambda>t. p2 (t + (t2 - t1))) rdy # tr') blks2 blks'"
+      using combine_blocks_waitE4[OF combine_blocks_wait2(1) c1]
+            combine_blocks_wait2(3,7) unfolding pre(3) by auto
+    have c3: "WaitBlk t2 (\<lambda>\<tau>. ParState (if \<tau> < t1 then p1 \<tau> else p2 (\<tau> - t1)) (hist2 \<tau>)) rdy' =
+              WaitBlk (t1 + (t2 - t1)) (\<lambda>\<tau>. ParState (if \<tau> < t1 then p1 \<tau> else p2 (\<tau> - t1)) (hist2 \<tau>)) rdy'"
       by auto
-    have c4: "d2 - (t2 - t1) = t1 + d2 - t2"
-      by auto
-    have c5: "(\<lambda>t\<in>{0..d2-(t2-t1)}. restrict p2 {0..d2} (t + (t2 - t1))) =
-              (\<lambda>\<tau>\<in>{0..t1+d2-t2}. if 0 \<le> \<tau> + t2 \<and> \<tau> + t2 \<le> t1 + d2 then if \<tau> + t2 < t1 then p1 (\<tau> + t2) else p2 (\<tau> + t2 - t1) else undefined)"
-      unfolding c4 apply (rule restrict_ext)
-      using combine_blocks_wait2 apply auto
-      by (simp add: group_cancel.sub1)
+    have c4: "WaitBlk (d2 - (t2 - t1)) (\<lambda>t. p2 (t + (t2 - t1))) rdy =
+              WaitBlk (t1 + d2 - t2) (\<lambda>\<tau>. if \<tau> + t2 < t1 then p1 (\<tau> + t2) else p2 (\<tau> + t2 - t1)) rdy"
+      apply (auto simp add: WaitBlk_def)
+      apply (rule ext) using c1 pre(1) by (simp add: add_diff_eq)
     show ?thesis
       unfolding c2(1)
-      apply (rule exI[where x="WaitBlock t2 (\<lambda>\<tau>\<in>{0..t2}. ParState (if \<tau> < t1 then p1 \<tau> else p2 (\<tau> - t1)) (hist2 \<tau>)) rdy' # blks'"])
+      apply (rule exI[where x="WaitBlk t2 (\<lambda>\<tau>. ParState (if \<tau> < t1 then p1 \<tau> else p2 (\<tau> - t1)) (hist2 \<tau>)) rdy' # blks'"])
       apply auto
       subgoal
         unfolding combine_blocks_wait2(6) c3
         apply (rule reduce_trace_merge')
-        using combine_blocks_wait2(4,8-10) c1 by auto
+        using combine_blocks_wait2(4,9-11) restrict_cong_to_eq[OF pre(2)] c1 pre(1) by auto
       subgoal
+        unfolding pre(1)
         apply (rule combine_blocks.combine_blocks_wait3)
-        using combine_blocks_wait2(3-10) that c2
-        unfolding c5 unfolding c4 by auto
+        using combine_blocks_wait2(3-11) that c2
+        unfolding pre c4 by auto
       done
   qed
   show ?case
     using a b c by fastforce
 next
-  case (combine_blocks_wait3 comms t1 t2 blks2 blks rdy2 hist hist2 rdy')
-  have "\<exists>tr''.
-   reduce_trace blks tr'' \<and>
-   combine_blocks comms (WaitBlock (t1 - t2 + d2) (\<lambda>\<tau>\<in>{0..t1-t2+d2}. if \<tau> < t1 - t2 then p1 (\<tau> + t2) else p2 (\<tau> - (t1 - t2))) rdy # tr') blks2 tr''"
+  case (combine_blocks_wait3 comms t1 t2 hist1 rdy1 blks2 blks rdy2 hist hist2 rdy')
+  have pre: "d1 = t1" "restrict hist1 {0..t1} = restrict p1 {0..t1}" "rdy1 = rdy"
+    using combine_blocks_wait3(8) unfolding WaitBlk_def by auto
+  have pre2: "WaitBlk (t1 - t2) (\<lambda>\<tau>. hist1 (\<tau> + t2)) rdy = WaitBlk (t1 - t2) (\<lambda>\<tau>. p1 (\<tau> + t2)) rdy"
+    apply (auto simp add: WaitBlk_def) apply (rule ext)
+    using restrict_cong_to_eq[OF pre(2)] combine_blocks_wait3.hyps(5) by auto
+  have "\<exists>tr''. reduce_trace blks tr'' \<and>
+          combine_blocks comms (WaitBlk (t1 - t2 + d2) (\<lambda>\<tau>. if \<tau> < t1 - t2 then p1 (\<tau> + t2) else p2 (\<tau> - (t1 - t2))) rdy # tr') blks2 tr''"
     apply (rule combine_blocks_wait3(2))
-    using combine_blocks_wait3(3-10) by auto
+    using combine_blocks_wait3(3-11) restrict_cong_to_eq[OF pre(2)] pre(1,3) pre2 by auto
   then obtain tr'' where a:
     "reduce_trace blks tr''"
-    "combine_blocks comms (WaitBlock (t1 - t2 + d2) (\<lambda>\<tau>\<in>{0..t1-t2+d2}. if \<tau> < t1 - t2 then p1 (\<tau> + t2) else p2 (\<tau> - (t1 - t2))) rdy # tr') blks2 tr''"
+    "combine_blocks comms (WaitBlk (t1 - t2 + d2) (\<lambda>\<tau>. if \<tau> < t1 - t2 then p1 (\<tau> + t2) else p2 (\<tau> - (t1 - t2))) rdy # tr') blks2 tr''"
     by auto
-  have b: "t1 - t2 + d2 = t1 + d2 - t2"
-    by auto
-  have b2: "\<tau> - (t1 - t2) = \<tau> + t2 - t1" for \<tau>
-    by auto
-  have c: "WaitBlock (t1 - t2 + d2) (\<lambda>\<tau>\<in>{0..t1-t2+d2}. if \<tau> < t1 - t2 then p1 (\<tau> + t2) else p2 (\<tau> - (t1 - t2))) rdy =
-           WaitBlock (t1 + d2 - t2) (\<lambda>\<tau>\<in>{0..t1+d2-t2}. (\<lambda>\<tau>\<in>{0..t1+d2}. if \<tau> < t1 then p1 \<tau> else p2 (\<tau> - t1)) (\<tau> + t2)) rdy"
-    unfolding b apply auto
-    apply (rule restrict_ext)
-    using combine_blocks_wait3(3-10) by (auto simp add: b2)
+  have c: "WaitBlk (t1 - t2 + d2) (\<lambda>\<tau>. if \<tau> < t1 - t2 then p1 (\<tau> + t2) else p2 (\<tau> - (t1 - t2))) rdy =
+           WaitBlk (d1 + d2 - t2) (\<lambda>\<tau>. if \<tau> + t2 < d1 then p1 (\<tau> + t2) else p2 (\<tau> + t2 - d1)) rdy"
+    apply (auto simp add: WaitBlk_def pre(1)) apply (rule ext)
+    by (simp add: diff_diff_eq2 pre(1))
+  have d: "WaitBlk t2 hist rdy' = WaitBlk t2 (\<lambda>\<tau>. ParState (if \<tau> < t1 then p1 \<tau> else p2 (\<tau> - t1)) (hist2 \<tau>)) rdy'"
+    unfolding WaitBlk_def apply (auto simp add: combine_blocks_wait3(4))
+    unfolding combine_blocks_wait3(6)
+    apply (rule restrict_combine_cong)
+    apply auto apply (rule ext) using restrict_cong_to_eq[OF pre(2)] \<open>t2 < t1\<close> by auto
   show ?case
-    apply (rule exI[where x="WaitBlock t2 hist rdy' # tr''"])
+    apply (rule exI[where x="WaitBlk t2 hist rdy' # tr''"])
     apply auto
     subgoal apply (rule reduce_trace_cons) by (rule a(1))
-    apply (rule combine_blocks.combine_blocks_wait3)
+    unfolding d apply (rule combine_blocks.combine_blocks_wait3)
     subgoal using a(2) unfolding c by auto
-    using combine_blocks_wait3(3-10) by auto
-qed
+    using combine_blocks_wait3(3-11) pre(1,3) by auto
+qed (auto simp add: WaitBlk_def)
 
 lemma combine_blocks_merge_right:
-  "combine_blocks chs tr1 (WaitBlock d1 (restrict p1 {0..d1}) rdy # WaitBlock d2 (restrict p2 {0..d2}) rdy # tr') tr \<Longrightarrow>
+  "combine_blocks chs tr1 (WaitBlk d1 p1 rdy # WaitBlk d2 p2 rdy # tr') tr \<Longrightarrow>
    p1 d1 = p2 0 \<Longrightarrow>
    d1 > 0 \<Longrightarrow> d2 > 0 \<Longrightarrow>
    \<exists>tr''. reduce_trace tr tr'' \<and>
-   combine_blocks chs tr1 (WaitBlock (d1 + d2) (\<lambda>\<tau>\<in>{0..d1+d2}. if \<tau> < d1 then p1 \<tau> else p2 (\<tau> - d1)) rdy # tr') tr''"
-proof (induct chs tr1 "WaitBlock d1 (restrict p1 {0..d1}) rdy # WaitBlock d2 (restrict p2 {0..d2}) rdy # tr'" tr
+   combine_blocks chs tr1 (WaitBlk (d1 + d2) (\<lambda>\<tau>. if \<tau> < d1 then p1 \<tau> else p2 (\<tau> - d1)) rdy # tr') tr''"
+proof (induct chs tr1 "WaitBlk d1 p1 rdy # WaitBlk d2 p2 rdy # tr'" tr
        arbitrary: d1 p1 rule: combine_blocks.induct)
   case (combine_blocks_unpair1 ch comms blks1 blks ch_type v)
   then show ?case
     using combine_blocks.combine_blocks_unpair1 reduce_trace_cons by blast
 next
-  case (combine_blocks_wait1 comms blks1 blks rdy1 hist hist1 t rdy')
-  have a: "(\<lambda>\<tau>\<in>{0..d2}. if 0 \<le> \<tau> + t \<and> \<tau> \<le> d2 then if \<tau> + t < t then p1 (\<tau> + t) else p2 (\<tau> + t - t) else undefined) =
-           (\<lambda>\<tau>\<in>{0..d2}. p2 \<tau>)" if "t > 0"
+  case (combine_blocks_wait1 chs blks1 blks rdy1 rdy2 hist hist1 hist2 rdy' t)
+  have a: "t = d1" "restrict hist2 {0..t} = restrict p1 {0..t}" "rdy = rdy2"
+    using combine_blocks_wait1(6) unfolding WaitBlk_def by auto
+  have b: "(\<lambda>\<tau>\<in>{0..d2}. if \<tau> < 0 then p1 (\<tau> + t) else p2 (\<tau> + t - d1)) = (\<lambda>\<tau>\<in>{0..d2}. p2 \<tau>)"
     apply (rule restrict_ext)
-    using combine_blocks_wait1 that by auto
+    by (auto simp add: a(1))
+  have c: "WaitBlk t hist rdy' = WaitBlk t (\<lambda>\<tau>. ParState (hist1 \<tau>) (if \<tau> < d1 then p1 \<tau> else p2 (\<tau> - d1))) rdy'"
+    unfolding WaitBlk_def apply (auto simp add: combine_blocks_wait1(4))
+    apply (rule ext)
+    using restrict_combine_cong[OF _ a(2)]
+    by (auto simp add: a combine_blocks_wait1(7))
   show ?case
-    apply (rule exI[where x="WaitBlock t hist rdy' # blks"])
-    apply auto
+    apply (rule exI[where x="WaitBlk t hist rdy' # blks"])
+    apply auto unfolding c
     apply (rule combine_blocks_wait2)
-    subgoal apply (auto simp add: combine_blocks_wait1)
-      unfolding a
-      by (simp add: a combine_blocks_wait1.hyps(1) combine_blocks_wait1.prems(2))
-    using combine_blocks_wait1 by auto
+    subgoal
+      apply (auto simp add: a(1) WaitBlk_def b)
+      using combine_blocks_wait1(1)[unfolded WaitBlk_def] by auto
+    using combine_blocks_wait1 a by auto
 next
-  case (combine_blocks_wait2 comms blks1 t2 t1 blks rdy1 hist hist1 rdy')
-  have "\<exists>tr''.
-   reduce_trace blks tr'' \<and>
-   combine_blocks comms blks1 (WaitBlock (t2 - t1 + d2) (\<lambda>\<tau>\<in>{0..t2-t1+d2}. if \<tau> < t2 - t1 then p1 (\<tau> + t1) else p2 (\<tau> - (t2 - t1))) rdy # tr') tr''"
+  case (combine_blocks_wait2 comms blks1 t2 t1 hist2 rdy2 blks rdy1 hist hist1 rdy')
+  have pre: "d1 = t2" "restrict hist2 {0..t2} = restrict p1 {0..t2}" "rdy2 = rdy"
+    using combine_blocks_wait2(8) unfolding WaitBlk_def by auto
+  have pre2: "WaitBlk (t2 - t1) (\<lambda>\<tau>. hist2 (\<tau> + t1)) rdy = WaitBlk (t2 - t1) (\<lambda>\<tau>. p1 (\<tau> + t1)) rdy"
+    apply (auto simp add: WaitBlk_def) apply (rule ext)
+    using restrict_cong_to_eq[OF pre(2)] combine_blocks_wait2.hyps(5) by auto
+  have "\<exists>tr''. reduce_trace blks tr'' \<and>
+          combine_blocks comms blks1 (WaitBlk (t2 - t1 + d2) (\<lambda>\<tau>. if \<tau> < t2 - t1 then p1 (\<tau> + t1) else p2 (\<tau> - (t2 - t1))) rdy # tr') tr''"
     apply (rule combine_blocks_wait2(2))
-    using combine_blocks_wait2(3-10) by auto
+    using combine_blocks_wait2(3-11) restrict_cong_to_eq[OF pre(2)] pre(1,3) pre2 by auto
   then obtain tr'' where a:
     "reduce_trace blks tr''"
-    "combine_blocks comms blks1 (WaitBlock (t2 - t1 + d2) (\<lambda>\<tau>\<in>{0..t2-t1+d2}. if \<tau> < t2 - t1 then p1 (\<tau> + t1) else p2 (\<tau> - (t2 - t1))) rdy # tr') tr''"
+    "combine_blocks comms blks1 (WaitBlk (t2 - t1 + d2) (\<lambda>\<tau>. if \<tau> < t2 - t1 then p1 (\<tau> + t1) else p2 (\<tau> - (t2 - t1))) rdy # tr') tr''"
     by auto
-  have b: "t2 - t1 + d2 = t2 + d2 - t1"
-    by auto
-  have b2: "\<tau> - (t2 - t1) = \<tau> + t1 - t2" for \<tau>
-    by auto
-  have c: "WaitBlock (t2 - t1 + d2) (\<lambda>\<tau>\<in>{0..t2-t1+d2}. if \<tau> < t2 - t1 then p1 (\<tau> + t1) else p2 (\<tau> - (t2 - t1))) rdy =
-           WaitBlock (t2 + d2 - t1) (\<lambda>\<tau>\<in>{0..t2+d2-t1}. (\<lambda>\<tau>\<in>{0..t2+d2}. if \<tau> < t2 then p1 \<tau> else p2 (\<tau> - t2)) (\<tau> + t1)) rdy"
-    unfolding b apply auto
-    apply (rule restrict_ext)
-    using combine_blocks_wait2(3-10) by (auto simp add: b2)
+  have c: "WaitBlk (t2 - t1 + d2) (\<lambda>\<tau>. if \<tau> < t2 - t1 then p1 (\<tau> + t1) else p2 (\<tau> - (t2 - t1))) rdy =
+           WaitBlk (d1 + d2 - t1) (\<lambda>\<tau>. if \<tau> + t1 < d1 then p1 (\<tau> + t1) else p2 (\<tau> + t1 - d1)) rdy"
+    apply (auto simp add: WaitBlk_def pre(1)) apply (rule ext)
+    by (simp add: diff_diff_eq2 pre(1))
+  have d: "WaitBlk t1 hist rdy' = WaitBlk t1 (\<lambda>\<tau>. ParState (hist1 \<tau>) (if \<tau> < t2 then p1 \<tau> else p2 (\<tau> - t2))) rdy'"
+    unfolding WaitBlk_def apply (auto simp add: combine_blocks_wait2(4))
+    unfolding combine_blocks_wait2(6)
+    apply (rule restrict_combine_cong)
+    apply auto apply (rule ext) using restrict_cong_to_eq[OF pre(2)] \<open>t1 < t2\<close> by auto
   show ?case
-    apply (rule exI[where x="WaitBlock t1 hist rdy' # tr''"])
+    apply (rule exI[where x="WaitBlk t1 hist rdy' # tr''"])
     apply auto
     subgoal apply (rule reduce_trace_cons) by (rule a(1))
-    apply (rule combine_blocks.combine_blocks_wait2)
+    unfolding d apply (rule combine_blocks.combine_blocks_wait2)
     subgoal using a(2) unfolding c by auto
-    using combine_blocks_wait2(3-10) by auto
+    using combine_blocks_wait2(3-11) pre(1,3) by auto
 next
-  case (combine_blocks_wait3 comms t1 t2 hist1 rdy1 blks1 blks hist rdy')
+  case (combine_blocks_wait3 comms t1 t2 hist1 rdy1 blks1 blks rdy2 hist hist2 rdy')
+  have pre: "d1 = t2" "restrict hist2 {0..t2} = restrict p1 {0..t2}" "rdy2 = rdy"
+    using combine_blocks_wait3(8) unfolding WaitBlk_def by auto
   have a: ?case if "t2 + d2 = t1"
   proof -
     have a1: "t1 - t2 = d2"
       using that by auto
     obtain blks' where a2:
-      "blks = WaitBlock d2 (\<lambda>t\<in>{0..d2}. ParState ((\<lambda>\<tau>\<in>{0..d2}. hist1 (\<tau> + t2)) t) (restrict p2 {0..d2} t)) rdy' # blks'"
+      "blks = WaitBlk d2 (\<lambda>t. ParState (hist1 (t + t2)) (p2 t)) rdy' # blks'"
       "combine_blocks comms blks1 tr' blks'"
       using combine_blocks_waitE2[OF combine_blocks_wait3(1)[unfolded a1]]
-            combine_blocks_wait3(3,7) by auto
+            combine_blocks_wait3(3,7) pre(3) by auto
     show ?thesis
       unfolding a2(1)
-      apply (rule exI[where x="WaitBlock (t2 + d2) (\<lambda>\<tau>\<in>{0..t2+d2}. ParState (hist1 \<tau>) (if \<tau> < t2 then p1 \<tau> else p2 (\<tau> - t2))) rdy' # blks'"])
+      apply (rule exI[where x="WaitBlk (t2 + d2) (\<lambda>\<tau>. ParState (hist1 \<tau>) (if \<tau> < t2 then p1 \<tau> else p2 (\<tau> - t2))) rdy' # blks'"])
       apply auto
       subgoal
         unfolding combine_blocks_wait3(6)
         apply (rule reduce_trace_merge')
-        using combine_blocks_wait3(8-10) by auto
+        using combine_blocks_wait3(9-11) restrict_cong_to_eq[OF pre(2)] pre(1) by auto
       subgoal
-        unfolding that
+        unfolding pre(1) that
         apply (rule combine_blocks.combine_blocks_wait1)
-        using combine_blocks_wait3(3,7) a2(2) by auto
+        using combine_blocks_wait3(3,7) a2(2) pre(3) by auto
       done
   qed
   have b: ?case if "t2 + d2 < t1"
@@ -1748,68 +1816,62 @@ next
     have b1: "d2 < t1 - t2"
       using that by auto
     obtain blks' where b2:
-      "blks = WaitBlock d2 (\<lambda>t\<in>{0..d2}. ParState ((\<lambda>\<tau>\<in>{0..t1-t2}. hist1 (\<tau> + t2)) t) (restrict p2 {0..d2} t)) rdy' # blks'"
-      "combine_blocks comms (WaitBlock (t1-t2-d2) (\<lambda>t\<in>{0..t1-t2-d2}. (\<lambda>\<tau>\<in>{0..t1-t2}. hist1 (\<tau> + t2)) (t + d2)) rdy1 # blks1) tr' blks'"
-      using combine_blocks_waitE4[OF combine_blocks_wait3(1) b1 combine_blocks_wait3(3)]
-            combine_blocks_wait3(7) by auto
-    have b3: "t1 - t2 - d2 = t1 - (t2 + d2)"
-      by auto
-    have b4:
-      "(\<lambda>t\<in>{0..t1-t2-d2}. (\<lambda>\<tau>\<in>{0..t1-t2}. hist1 (\<tau> + t2)) (t + d2)) = (\<lambda>\<tau>\<in>{0..t1-(t2+d2)}. hist1 (\<tau> + (t2 + d2)))"
-      unfolding b3 apply (rule restrict_ext)
-      apply auto
-       apply (metis add.assoc add.commute)
-      using combine_blocks_wait3.prems(3) by auto
+      "blks = WaitBlk d2 (\<lambda>t. ParState (hist1 (t + t2)) (p2 t)) rdy' # blks'"
+      "combine_blocks comms (WaitBlk (t1 - t2 - d2) (\<lambda>t. hist1 (t + d2 + t2)) rdy1 # blks1) tr' blks'"
+      using combine_blocks_waitE4[OF combine_blocks_wait3(1,11) b1]
+            combine_blocks_wait3(3,7) unfolding pre(3) by auto
+    have b3: "WaitBlk (t1 - t2 - d2) (\<lambda>t. hist1 (t + d2 + t2)) rdy1 = WaitBlk (t1 - (t2 + d2)) (\<lambda>\<tau>. hist1 (\<tau> + (t2 + d2))) rdy1"
+      apply (auto simp add: WaitBlk_def)
+      apply (rule ext) by (auto simp add: add.commute add.left_commute)
     show ?thesis
       unfolding b2(1)
-      apply (rule exI[where x="WaitBlock (t2 + d2) (\<lambda>\<tau>\<in>{0..t2+d2}. ParState (hist1 \<tau>) (if \<tau> < t2 then p1 \<tau> else p2 (\<tau> - t2))) rdy' # blks'"])
+      apply (rule exI[where x="WaitBlk (t2 + d2) (\<lambda>\<tau>. ParState (hist1 \<tau>) (if \<tau> < t2 then p1 \<tau> else p2 (\<tau> - t2))) rdy' # blks'"])
       apply auto
       subgoal
         unfolding combine_blocks_wait3(6)
         apply (rule reduce_trace_merge')
-        using combine_blocks_wait3(8-10) b1 by auto
+        using combine_blocks_wait3(9-11) restrict_cong_to_eq[OF pre(2)] b1 pre(1) by auto
       subgoal
+        unfolding pre(1)
         apply (rule combine_blocks.combine_blocks_wait3)
-        using combine_blocks_wait3(3,7-10) that b2(2)
-        unfolding b4 unfolding b3 by auto
+        using combine_blocks_wait3(3,7-11) that b2(2)
+        unfolding b3 pre by auto
       done
   qed
   have c: ?case if "t2 + d2 > t1"
   proof -
-    have c1: "t1 - t2 < d2"
-      using that by auto
+    have c1: "0 < t1 - t2" "t1 - t2 < d2"
+      using that combine_blocks_wait3(4) by auto
     obtain blks' where c2:
-      "blks = WaitBlock (t1 - t2) (\<lambda>t\<in>{0..t1-t2}. ParState ((\<lambda>\<tau>\<in>{0..t1-t2}. hist1 (\<tau> + t2)) t) (restrict p2 {0..d2} t)) rdy' # blks'"
-      "combine_blocks comms blks1 (WaitBlock (d2 - (t1 - t2)) (\<lambda>t\<in>{0..d2-(t1-t2)}. restrict p2 {0..d2} (t + (t1 - t2))) rdy # tr') blks'"
-      using combine_blocks_waitE3[OF combine_blocks_wait3(1) c1 combine_blocks_wait3(3)]
-            combine_blocks_wait3(7) by auto
-    have c3: "WaitBlock t1 (\<lambda>\<tau>\<in>{0..t1}. ParState (hist1 \<tau>) (if \<tau> < t2 then p1 \<tau> else p2 (\<tau> - t2))) rdy' =
-              WaitBlock (t2 + (t1 - t2)) (\<lambda>\<tau>\<in>{0..t2+(t1-t2)}. ParState (hist1 \<tau>) (if \<tau> < t2 then p1 \<tau> else p2 (\<tau> - t2))) rdy'"
+      "blks = WaitBlk (t1 - t2) (\<lambda>t. ParState (hist1 (t + t2)) (p2 t)) rdy' # blks'"
+      "combine_blocks comms blks1 (WaitBlk (d2 - (t1 - t2)) (\<lambda>t. p2 (t + (t1 - t2))) rdy # tr') blks'"
+      using combine_blocks_waitE3[OF combine_blocks_wait3(1) c1]
+            combine_blocks_wait3(3,7) unfolding pre(3) by auto
+    have c3: "WaitBlk t1 (\<lambda>\<tau>. ParState (hist1 \<tau>) (if \<tau> < t2 then p1 \<tau> else p2 (\<tau> - t2))) rdy' =
+              WaitBlk (t2 + (t1 - t2)) (\<lambda>\<tau>. ParState (hist1 \<tau>) (if \<tau> < t2 then p1 \<tau> else p2 (\<tau> - t2))) rdy'"
       by auto
-    have c4: "d2 - (t1 - t2) = t2 + d2 - t1"
-      by auto
-    have c5: "(\<lambda>t\<in>{0..d2-(t1-t2)}. restrict p2 {0..d2} (t + (t1 - t2))) =
-              (\<lambda>\<tau>\<in>{0..t2+d2-t1}. if 0 \<le> \<tau> + t1 \<and> \<tau> + t1 \<le> t2 + d2 then if \<tau> + t1 < t2 then p1 (\<tau> + t1) else p2 (\<tau> + t1 - t2) else undefined)"
-      unfolding c4 apply (rule restrict_ext)
-      using combine_blocks_wait3 apply auto
-      by (simp add: group_cancel.sub1)
+    have c4: "WaitBlk (d2 - (t1 - t2)) (\<lambda>t. p2 (t + (t1 - t2))) rdy =
+              WaitBlk (t2 + d2 - t1) (\<lambda>\<tau>. if \<tau> + t1 < t2 then p1 (\<tau> + t1) else p2 (\<tau> + t1 - t2)) rdy"
+      apply (auto simp add: WaitBlk_def)
+      apply (rule ext) using c1 pre(1) by (simp add: add_diff_eq)
     show ?thesis
       unfolding c2(1)
-      apply (rule exI[where x="WaitBlock t1 (\<lambda>\<tau>\<in>{0..t1}. ParState (hist1 \<tau>) (if \<tau> < t2 then p1 \<tau> else p2 (\<tau> - t2))) rdy' # blks'"])
+      apply (rule exI[where x="WaitBlk t1 (\<lambda>\<tau>. ParState (hist1 \<tau>) (if \<tau> < t2 then p1 \<tau> else p2 (\<tau> - t2))) rdy' # blks'"])
       apply auto
       subgoal
         unfolding combine_blocks_wait3(6) c3
         apply (rule reduce_trace_merge')
-        using combine_blocks_wait3(4,8-10) c1 by auto
+        using combine_blocks_wait3(4,9-11) restrict_cong_to_eq[OF pre(2)] c1 pre(1) by auto
       subgoal
+        unfolding pre(1)
         apply (rule combine_blocks.combine_blocks_wait2)
-        using combine_blocks_wait3(3-10) that c2
-        unfolding c5 unfolding c4 by auto
+        using combine_blocks_wait3(3-11) that c2
+        unfolding pre c4 by auto
       done
   qed
   show ?case
     using a b c by fastforce
-qed
+qed (auto simp add: WaitBlk_def)
 
 
 lemma combine_blocks_equiv_left:
@@ -1886,23 +1948,23 @@ proof (induction p s "Some ev" p2 s2 arbitrary: ev evs s3 rule: par_small_step.i
     using SingleS(2) apply (elim SingleE)
     by (metis SingleB SingleS.hyps gstate.inject(1) small1_big_continue2)
 next
-  case (ParDelayS rdy1 rdy2 hist hist1 hist2 t rdy p1 s1 p2 s2 p3 s3' p4 s4 chs)
-  have a: "\<exists>evs'. reduce_trace (WaitBlock t hist rdy # evs) evs' \<and>
+  case (ParDelayS rdy1 rdy2 hist hist1 hist2 rdy p1 s1 t p2 s2 p3 s3' p4 s4 chs)
+  have a: "\<exists>evs'. reduce_trace (WaitBlk t hist rdy # evs) evs' \<and>
                   par_big_step (Parallel p1 chs p3) (ParState s1 s3') evs' (ParState s12 s22)"
     if aH: "s3 = ParState s12 s22"
        "par_big_step p2 s2 tr1 s12"
        "par_big_step p4 s4 tr2 s22"
        "combine_blocks chs tr1 tr2 evs" for s12 s22 tr1 tr2
   proof -
-    obtain evs1 where b: "reduce_trace (WaitBlock t hist1 rdy1 # tr1) evs1" "par_big_step p1 s1 evs1 s12"
+    obtain evs1 where b: "reduce_trace (WaitBlk t hist1 rdy1 # tr1) evs1" "par_big_step p1 s1 evs1 s12"
       using ParDelayS(5)[OF aH(2)] by auto
-    obtain evs2 where c: "reduce_trace (WaitBlock t hist2 rdy2 # tr2) evs2" "par_big_step p3 s3' evs2 s22"
+    obtain evs2 where c: "reduce_trace (WaitBlk t hist2 rdy2 # tr2) evs2" "par_big_step p3 s3' evs2 s22"
       using ParDelayS(7)[OF aH(3)] by auto
-    have d: "combine_blocks chs (WaitBlock t hist1 rdy1 # tr1) (WaitBlock t hist2 rdy2 # tr2) (WaitBlock t hist rdy # evs)"
+    have d: "combine_blocks chs (WaitBlk t hist1 rdy1 # tr1) (WaitBlk t hist2 rdy2 # tr2) (WaitBlk t hist rdy # evs)"
       apply (rule combine_blocks_wait1[OF aH(4)])
       using ParDelayS by auto
     obtain tr' where e:
-      "reduce_trace (WaitBlock t hist rdy # evs) tr'"
+      "reduce_trace (WaitBlk t hist rdy # evs) tr'"
       "combine_blocks chs evs1 evs2 tr'"
       using b(1) c(1) d combine_blocks_equiv by blast
     show ?thesis
