lunarlander_sl/ExampleContinuous.thy
@@ -38,17 +38,17 @@ theorem Valid_interrupt_InIn:
     {\<lambda>s tr. (\<forall>v. Q1 (s(var1 := v)) (tr @ [InBlock ch1 v])) \<and>
             (\<forall>d>0. \<forall>p v. ODEsol ode p d \<longrightarrow> p 0 = s \<longrightarrow>
                 (\<forall>t. 0 \<le> t \<and> t < d \<longrightarrow> b (p t)) \<longrightarrow>
-                Q1 ((p d)(var1 := v)) (tr @ [WaitBlock d (\<lambda>\<tau>\<in>{0..d}. State (p \<tau>)) ({}, {ch1, ch2}),
+                Q1 ((p d)(var1 := v)) (tr @ [WaitBlk d (\<lambda>\<tau>. State (p \<tau>)) ({}, {ch1, ch2}),
                                              InBlock ch1 v])) \<and>
             (\<forall>v. Q2 (s(var2 := v)) (tr @ [InBlock ch2 v])) \<and>
             (\<forall>d>0. \<forall>p v. ODEsol ode p d \<longrightarrow> p 0 = s \<longrightarrow>
                 (\<forall>t. 0 \<le> t \<and> t < d \<longrightarrow> b (p t)) \<longrightarrow>
-                Q2 ((p d)(var2 := v)) (tr @ [WaitBlock d (\<lambda>\<tau>\<in>{0..d}. State (p \<tau>)) ({}, {ch1, ch2}),
+                Q2 ((p d)(var2 := v)) (tr @ [WaitBlk d (\<lambda>\<tau>. State (p \<tau>)) ({}, {ch1, ch2}),
                                              InBlock ch2 v])) \<and>
             (\<not>b s \<longrightarrow> R s tr) \<and>
             (\<forall>d>0. \<forall>p. ODEsol ode p d \<longrightarrow> p 0 = s \<longrightarrow>
                 (\<forall>t. 0 \<le> t \<and> t < d \<longrightarrow> b (p t)) \<longrightarrow> \<not>b (p d) \<longrightarrow>
-                R (p d) (tr @ [WaitBlock d (\<lambda>\<tau>\<in>{0..d}. State (p \<tau>)) ({}, {ch1, ch2})]))}
+                R (p d) (tr @ [WaitBlk d (\<lambda>\<tau>. State (p \<tau>)) ({}, {ch1, ch2})]))}
       Interrupt ode b [(ch1[?]var1, p1), (ch2[?]var2, p2)]
     {R}"
   apply (rule Valid_interrupt)
